WIP big re-specification, following discussion with Jean

theories/case_studies/multiuser_kvs/kvs_preamble.v
@@ -5,73 +5,24 @@ From griotte Require Import proofmode.
 From griotte Require Import logrel rules.
 From griotte Require Import switcher kvs.
 
-Definition kvs_entry : Type := option (Z * Word).
+
+Definition user_key_t := Z.
+Definition map_key_t := Z.
+Definition full_key_t := Z.
+
+Definition kvs_physical_entry : Type := option (full_key_t * Word).
 Definition kvs_dom : gset nat := set_seq 0 SIZE_MAP.
-Definition kvs_map : Type := gmap nat kvs_entry.
+Definition kvs_physical_map : Type := gmap nat kvs_physical_entry.
 
-Definition kvs_user_map : Type := gmap Z Word.
-Definition kvs_logical_map : Type := gmap Z kvs_user_map.
 
-(* CMRA for KVS *)
-Class kvsG Σ :=
-  KvsG {
-      kvs_genG :: gen_heapGS nat kvs_entry Σ;
-      kvs_user_genG :: gen_heapGS Z kvs_user_map Σ;
-    }.
-
-Notation "'↪●KVS_USERS' m" :=
-  ( gen_heap_interp (L:=Z) (V:= kvs_user_map) m )%I (at level 20) : bi_scope.
-
-Notation "uk '↦(KVS_USER)[' dq ']' umap" :=
-  (pointsto (L:=Z) (V:= kvs_user_map) uk dq umap)%I (at level 20) : bi_scope.
-Notation "uk '↦(KVS_USER)' umap" :=
-  (uk ↦(KVS_USER)[ (DfracOwn 1) ] umap)%I (at level 20) : bi_scope.
-
-Lemma kvs_logical_kvs_valid `{kvsG} (uk : Z) (m : kvs_logical_map) (umap : kvs_user_map) :
-  ↪●KVS_USERS m  -∗ uk ↦(KVS_USER) umap -∗ ⌜ m !! uk = Some umap ⌝.
-Proof.
-  iIntros "Hauth Hfrag".
-  by iDestruct (gen_heap_valid with "Hauth Hfrag") as "%Hvalid".
-Qed.
-
-Lemma kvs_logical_kvs_update `{kvsG} (uk : Z) (m : kvs_logical_map) (umap umap' : kvs_user_map) :
-  ↪●KVS_USERS m -∗ uk ↦(KVS_USER) umap
-  ==∗
-  ↪●KVS_USERS (<[uk := umap']> m) ∗ uk ↦(KVS_USER) umap'.
-Proof.
-  iIntros "Hauth Hfrag".
-  by iMod (gen_heap_update m uk _ umap' with "Hauth Hfrag") as "[$ $]".
-Qed.
-
-Definition kvs_frag_idx_frac `{kvsG} (idx : nat) (k : Z) (w : Word) (q : dfrac) : iProp Σ :=
-  (pointsto (L:=nat) (V:=kvs_entry) idx q (Some (k,w))).
-Notation "k '⤇(KVS){' q '}[' idx  ']' w" :=
-  (kvs_frag_idx_frac idx k w q) (at level 20) : bi_scope.
-Notation "k '⤇(KVS){' q '}[' idx  ']' -" :=
-  (∃ w, kvs_frag_idx_frac idx k w q)%I (at level 20) : bi_scope.
-
-Notation "idx '⤇(KVS)' 'NONE'" :=
-  (pointsto (L:=nat) (V:=kvs_entry) idx (DfracOwn 1) None) (at level 20) : bi_scope.
-Notation "k '⤇(KVS)[' idx  ']' w" :=
-  (kvs_frag_idx_frac idx k w (DfracOwn 1)) (at level 20) : bi_scope.
-Notation "k '⤇(KVS)[' idx  ']' -" :=
-  (∃ w, kvs_frag_idx_frac idx k w (DfracOwn 1))%I (at level 20) : bi_scope.
-
-Definition kvs_frag `{kvsG} (k : Z ) (w : Word) : iProp Σ := ∃ idx, k ⤇(KVS)[ idx ] w.
-Notation "k '⤇(KVS)' w" := (kvs_frag k w) (at level 20) : bi_scope.
-Notation "k '⤇(KVS)' -" := (∃ w, kvs_frag k w)%I (at level 20) : bi_scope.
-
-Notation "●(KVS) m" := (gen_heap_interp (m : kvs_map)) (at level 20) : bi_scope.
-
-Section KVS_preamble.
+Section KVS_physical_map.
   Context
     {Σ:gFunctors}
     {ceriseg:ceriseG Σ}
-    {kvsg:kvsG Σ}
     `{MP: MachineParameters}
   .
 
-  Definition kvs_keys (m : kvs_map) : list Z :=
+  Definition kvs_keys (pkvs : kvs_physical_map) : list full_key_t :=
     map_fold (
         (fun _ opt_kv acc =>
            match opt_kv with
@@ -81,36 +32,68 @@ Section KVS_preamble.
         )
       )
       []
-      m.
+      pkvs.
 
-  Definition wf_kvs_map (m : kvs_map) : Prop :=
-    dom m = kvs_dom ∧ NoDup (kvs_keys m).
+  Definition wf_kvs_physical_map (pkvs : kvs_physical_map) : Prop :=
+    dom pkvs = kvs_dom ∧ NoDup (kvs_keys pkvs).
 
-  Definition option_pair_ASM (opt_kw : kvs_entry) (wuk wmk : Word) :=
+  Definition option_pair_ASM_Some (k : full_key_t) (w : Word) :=
+    [ WInt ASM_SOME; WInt k; w].
+  Definition option_pair_ASM_None (wuk wmk : Word) :=
+    [ WInt ASM_NONE; wuk; wmk].
+
+  Definition option_pair_ASM (opt_kw : kvs_physical_entry) (wuk wmk : Word) :=
     match opt_kw with
-    | None => [WInt ASM_NONE; wuk; wmk]
-    | Some (k, w) => [ WInt ASM_SOME; WInt k; w]
+    | None => option_pair_ASM_None wuk wmk
+    | Some (k, w) => option_pair_ASM_Some k w
     end.
 
-  Definition isKVS_entry (a : Addr) (idx : nat) (opt_kw : kvs_entry) : iProp Σ :=
+  Definition physical_kvs_entry (a : Addr) (idx : nat) (opt_kw : kvs_physical_entry) : iProp Σ :=
+    let a_opt_idx := (a ^+ (ASM_SIZEOF_KVS_ENTRY*idx))%a in
+    let a_opt_idx_next := (a ^+ (ASM_SIZEOF_KVS_ENTRY * idx + ASM_SIZEOF_KVS_ENTRY))%a in
     ∃ (wuk wmk : Word),
-    [[ (a ^+ (ASM_SIZEOF_KVS_ENTRY*idx))%a, (a ^+ (ASM_SIZEOF_KVS_ENTRY * idx + ASM_SIZEOF_KVS_ENTRY))%a ]]
-      ↦ₐ [[ option_pair_ASM opt_kw wuk wmk ]]
-    ∗ (match opt_kw with | None => idx ⤇(KVS) NONE | Some _ => True end).
+      [[ a_opt_idx, a_opt_idx_next ]] ↦ₐ [[ option_pair_ASM opt_kw wuk wmk ]].
 
-  Lemma destruct_isKVS_entry_Some (a : Addr) (idx : nat) (k : Z) (w : Word) :
+  Definition physical_kvs_entry' (a : Addr) (idx : nat) (opt_kw : kvs_physical_entry) : iProp Σ :=
+    let a_opt := (a ^+ (ASM_SIZEOF_KVS_ENTRY*idx))%a in
+    let a_key := (a ^+ (ASM_SIZEOF_KVS_ENTRY*idx+1))%a in
+    let a_val := (a ^+ (ASM_SIZEOF_KVS_ENTRY*idx+2))%a in
+    ( a_opt ↦ₐ ( match opt_kw with | None => WInt ASM_NONE | Some _ => WInt ASM_SOME end ) ) ∗
+    ( match opt_kw with
+      | None =>       a_key ↦ₐ -
+      | Some (k,_) => a_key ↦ₐ WInt k
+      end ) ∗
+    ( match opt_kw with
+      | None =>       a_val ↦ₐ -
+      | Some (_,w) => a_val ↦ₐ w
+      end).
+
+  Definition physical_kvs_entry_some' (a : Addr) (idx : nat) (k : full_key_t) (w : Word) : iProp Σ :=
+    let a_opt := (a ^+ (ASM_SIZEOF_KVS_ENTRY*idx))%a in
+    let a_key := (a ^+ (ASM_SIZEOF_KVS_ENTRY*idx+1))%a in
+    let a_val := (a ^+ (ASM_SIZEOF_KVS_ENTRY*idx+2))%a in
+    ( a_opt ↦ₐ WInt ASM_SOME ∗
+      a_key ↦ₐ WInt k ∗
+      a_val ↦ₐ w).
+
+  Definition physical_kvs_entry_none' (a : Addr) (idx : nat) : iProp Σ :=
+    let a_opt := (a ^+ (ASM_SIZEOF_KVS_ENTRY*idx))%a in
+    let a_key := (a ^+ (ASM_SIZEOF_KVS_ENTRY*idx+1))%a in
+    let a_val := (a ^+ (ASM_SIZEOF_KVS_ENTRY*idx+2))%a in
+    ( a_opt ↦ₐ WInt ASM_NONE ∗
+      a_key ↦ₐ - ∗
+      a_val ↦ₐ -).
+
+  Lemma destruct_physical_kvs_entry_some (a : Addr) (idx : nat) (k : full_key_t) (w : Word) :
   (a ^+ ASM_SIZEOF_KVS_ENTRY * idx + ASM_SIZEOF_KVS_ENTRY)%a
   = Some (a ^+ (ASM_SIZEOF_KVS_ENTRY * idx + ASM_SIZEOF_KVS_ENTRY))%a
     ->
 
-    isKVS_entry a idx (Some (k, w)) ⊣⊢
-    ( (a ^+ (ASM_SIZEOF_KVS_ENTRY*idx))%a ↦ₐ WInt ASM_SOME ∗
-      (a ^+ (ASM_SIZEOF_KVS_ENTRY*idx+1))%a ↦ₐ WInt k ∗
-      (a ^+ (ASM_SIZEOF_KVS_ENTRY*idx+2))%a ↦ₐ w).
+    physical_kvs_entry a idx (Some (k, w)) ⊣⊢ physical_kvs_entry_some' a idx k w.
   Proof.
     intros H.
     iSplit; iIntros "H".
-    - iDestruct "H" as "(%&%&H&_)".
+    - iDestruct "H" as "(%&%&H)".
       iDestruct (region_pointsto_cons _ (a ^+ ((ASM_SIZEOF_KVS_ENTRY * idx)+1))%a with "H") as
         "[$ H]"; try solve_addr.
       iDestruct (region_pointsto_cons _ (a ^+ ((ASM_SIZEOF_KVS_ENTRY * idx)+2))%a with "H") as
@@ -119,7 +102,6 @@ Section KVS_preamble.
         "[$ H]"; try solve_addr.
     - iDestruct "H" as "(?&?&?)".
       iExists (WInt 0), (WInt 0).
-      iSplit; last done.
       iApply (region_pointsto_cons _ (a ^+ ((ASM_SIZEOF_KVS_ENTRY * idx)+1))%a)
       ; [solve_addr | solve_addr | iFrame].
       iApply (region_pointsto_cons _ (a ^+ ((ASM_SIZEOF_KVS_ENTRY * idx)+2))%a)
@@ -130,29 +112,23 @@ Section KVS_preamble.
       rewrite finz_seq_between_empty; done.
   Qed.
 
-  Lemma destruct_isKVS_entry_None (a : Addr) (idx : nat) :
-  (a ^+ ASM_SIZEOF_KVS_ENTRY * idx + ASM_SIZEOF_KVS_ENTRY)%a
-  = Some (a ^+ (ASM_SIZEOF_KVS_ENTRY * idx + ASM_SIZEOF_KVS_ENTRY))%a
+  Lemma destruct_physical_kvs_entry_None (a : Addr) (idx : nat) :
+    (a ^+ ASM_SIZEOF_KVS_ENTRY * idx + ASM_SIZEOF_KVS_ENTRY)%a
+    = Some (a ^+ (ASM_SIZEOF_KVS_ENTRY * idx + ASM_SIZEOF_KVS_ENTRY))%a
     ->
 
-    isKVS_entry a idx None ⊣⊢
-    ( (∃ wuk wmk,
-        ( (a ^+ (ASM_SIZEOF_KVS_ENTRY*idx))%a ↦ₐ WInt ASM_NONE ∗
-          (a ^+ (ASM_SIZEOF_KVS_ENTRY*idx+1))%a ↦ₐ wuk ∗
-          (a ^+ (ASM_SIZEOF_KVS_ENTRY*idx+2))%a ↦ₐ wmk))
-    ∗ idx ⤇(KVS) NONE).
+      physical_kvs_entry a idx None ⊣⊢ physical_kvs_entry_none' a idx.
   Proof.
     intros H.
     iSplit; iIntros "H".
-    - iDestruct "H" as "(%&%&H&$)".
-      iExists wuk, wmk.
+    - iDestruct "H" as "(%&%&H)".
       iDestruct (region_pointsto_cons _ (a ^+ ((ASM_SIZEOF_KVS_ENTRY * idx)+1))%a with "H") as
         "[$ H]"; try solve_addr.
       iDestruct (region_pointsto_cons _ (a ^+ ((ASM_SIZEOF_KVS_ENTRY * idx)+2))%a with "H") as
         "[$ H]"; try solve_addr.
       iDestruct (region_pointsto_cons _ (a ^+ ((ASM_SIZEOF_KVS_ENTRY * idx)+3))%a with "H") as
         "[$ H]"; try solve_addr.
-    - iDestruct "H" as "[  (%wuk&%wmk&?&?&?) $]".
+    - iDestruct "H" as "( ? & [%wuk ?] & [%wmk ?] )".
       iExists wuk, wmk.
       iApply (region_pointsto_cons _ (a ^+ ((ASM_SIZEOF_KVS_ENTRY * idx)+1))%a)
       ; [solve_addr | solve_addr | iFrame].
@@ -164,39 +140,413 @@ Section KVS_preamble.
       rewrite finz_seq_between_empty; done.
   Qed.
 
-  Lemma destruct_isKVS_entry (a : Addr) (idx : nat) (opt_kw : kvs_entry) :
+  Lemma destruct_physical_kvs_entry (a : Addr) (idx : nat) (opt_kw : kvs_physical_entry) :
   (a ^+ ASM_SIZEOF_KVS_ENTRY * idx + ASM_SIZEOF_KVS_ENTRY)%a
   = Some (a ^+ (ASM_SIZEOF_KVS_ENTRY * idx + ASM_SIZEOF_KVS_ENTRY))%a
     ->
 
-    isKVS_entry a idx opt_kw ⊣⊢
-        ( (a ^+ (ASM_SIZEOF_KVS_ENTRY*idx))%a
-            ↦ₐ ( match opt_kw with | None => WInt ASM_NONE | Some _ => WInt ASM_SOME end )
-          ∗
-          ( match opt_kw with
-            | None => (a ^+ (ASM_SIZEOF_KVS_ENTRY*idx+1))%a ↦ₐ -
-            | Some (k,_) => (a ^+ (ASM_SIZEOF_KVS_ENTRY*idx+1))%a ↦ₐ WInt k
-            end )
-          ∗
-          ( match opt_kw with
-            | None => (a ^+ (ASM_SIZEOF_KVS_ENTRY*idx+2))%a ↦ₐ -
-            | Some (_,w) => (a ^+ (ASM_SIZEOF_KVS_ENTRY*idx+2))%a ↦ₐ w
-            end )
-          ∗ (match opt_kw with | None => idx ⤇(KVS) NONE | Some _ => True end)
-        ).
+    physical_kvs_entry a idx opt_kw ⊣⊢ physical_kvs_entry' a idx opt_kw.
   Proof.
     intros H.
     destruct opt_kw as [ [k w] |]; cbn.
-    - rewrite destruct_isKVS_entry_Some; auto.
-      iSplit; [iIntros "($&$&$)"| iIntros "($&$&$&_)"].
-    - rewrite destruct_isKVS_entry_None; auto.
-      iSplit; iIntros "H"; eauto.
-      + iDestruct "H" as "[  (%&%&($&$&$)) $]".
-      + iDestruct "H" as "($ & [% $] & [% $] & $)".
+    - rewrite destruct_physical_kvs_entry_some; auto.
+    - rewrite destruct_physical_kvs_entry_None; auto.
   Qed.
 
-  Definition kvs_elem_of_logical_kvs (lm : kvs_logical_map) (uk mk : Z) ( w : Word ) :=
-    (∃ umap, lm !! uk = Some umap ∧  umap !! mk = Some w).
+  Definition is_physical_kvs (a : Addr) (pkvs : kvs_physical_map) : iProp Σ :=
+    ⌜ wf_kvs_physical_map pkvs ⌝ ∗ [∗ map] idx ↦ opt_kw ∈ pkvs, physical_kvs_entry a idx opt_kw.
+
+  Definition is_physical_kvs_open (a : Addr) (pkvs : kvs_physical_map) (open_idx : nat) : iProp Σ :=
+    ⌜ wf_kvs_physical_map pkvs ⌝ ∗
+    [∗ map] idx ↦ opt_kw ∈ (delete open_idx pkvs), physical_kvs_entry a idx opt_kw.
+
+
+  Lemma wf_kvs_indom_idx (m : kvs_physical_map) (idx : nat) :
+    idx ∈ dom m ->
+    wf_kvs_physical_map m ->
+    0 <= idx < SIZE_MAP.
+  Proof.
+    intros Hm_idx [Hkvs_dom _].
+    rewrite Hkvs_dom /kvs_dom in Hm_idx.
+    apply elem_of_set_seq in Hm_idx.
+    lia.
+  Qed.
+
+  Lemma wf_kvs_is_Some (m : kvs_physical_map) (idx : nat)  :
+    wf_kvs_physical_map m ->
+    0 <= idx < SIZE_MAP ->
+    is_Some (m !! idx).
+  Proof.
+    intros [Hkvs_dom _] Hidx.
+    apply elem_of_dom.
+    rewrite Hkvs_dom /kvs_dom.
+    by apply elem_of_set_seq.
+  Qed.
+
+  Lemma kvs_physical_map_indom_idx (pkvs : kvs_physical_map) (a : Addr) (idx : nat) :
+    idx ∈ dom pkvs ->
+    is_physical_kvs a pkvs -∗
+    ⌜ 0 <= idx < SIZE_MAP ⌝.
+  Proof.
+    iIntros (Hm_idx) "(%Hwf_kvs & _)"; iPureIntro.
+    by eapply wf_kvs_indom_idx.
+  Qed.
+
+  Lemma kvs_physical_map_open_in
+    (a : Addr) (pkvs : kvs_physical_map)
+    (idx : nat) (k : full_key_t) (w : Word) :
+
+    pkvs !! idx = Some (Some (k, w)) ->
+
+    is_physical_kvs a pkvs -∗
+    is_physical_kvs_open a pkvs idx ∗ physical_kvs_entry a idx (Some (k, w)).
+  Proof.
+    iIntros (Hpkvs_idx) "[%Hwf_pkvs HKVS]".
+    rewrite -{1}(insert_id pkvs idx (Some (k,w))); last done.
+    iDestruct (big_sepM_insert_delete with "HKVS") as "[$ HKVS]".
+    iFrame; eauto.
+  Qed.
+
+  Global Instance Permutation_Reflexive {A} : Reflexive (@Permutation A).
+  Proof. intros l ; done. Qed.
+
+  Global Instance Permutation_Transitive {A} : Transitive (@Permutation A).
+  Proof. intros l1 l2 l3 Hl12 Hl23; eapply Permutation_trans; done. Qed.
+
+  Global Instance Permutation_PreOrder {A} : PreOrder (@Permutation A).
+  Proof. split; apply _. Qed.
+
+  Local Instance Proper_get_kvs_key (opt_kv : kvs_physical_entry) :
+  Proper (Permutation ==> Permutation)
+    (λ acc : list Z, match opt_kv with
+                     | Some kv => kv.1 :: acc
+                     | None => acc
+                     end).
+  Proof. intros l1 l2 Hl; destruct opt_kv; auto. Qed.
+
+  Lemma kvs_keys_insert_None idx m :
+    m !! idx = None ->
+    kvs_keys (<[idx:=None]> m) ≡ₚ kvs_keys m.
+  Proof.
+    intros Hidx.
+    rewrite /kvs_keys.
+    setoid_rewrite map_fold_insert; auto; try apply _.
+    intros j1 j2 opt_kv1 opt_kv2 l Hk_neq Hj1 Hj2.
+    destruct opt_kv1, opt_kv2; auto.
+    econstructor.
+  Qed.
+
+  Lemma kvs_keys_insert_Some idx k w m :
+    m !! idx = None ->
+    kvs_keys (<[idx:=Some (k, w)]> m) ≡ₚ (k :: kvs_keys m).
+  Proof.
+    intros Hidx.
+    rewrite /kvs_keys.
+    setoid_rewrite map_fold_insert; auto; try apply _.
+    intros j1 j2 opt_kv1 opt_kv2 l Hk_neq Hj1 Hj2.
+    destruct opt_kv1, opt_kv2; auto.
+    econstructor.
+  Qed.
+
+  Lemma wf_kvs_neq (m : kvs_physical_map) (idx idx' : nat) (k k' : Z) (w w' : Word) :
+    wf_kvs_physical_map m ->
+    idx ≠ idx' ->
+    m !! idx = Some (Some (k, w)) ->
+    m !! idx' = Some (Some (k', w')) ->
+    k ≠ k'.
+  Proof.
+    intros [_ Hkvs_uniqueness] Hidx_ne Hm_idx Hm_idx'.
+    rewrite -(insert_id m idx (Some (k, w))) in Hkvs_uniqueness; last done.
+    rewrite -insert_delete_eq in Hkvs_uniqueness.
+    rewrite kvs_keys_insert_Some in Hkvs_uniqueness; last by simplify_map_eq.
+    rewrite -(insert_id (delete idx m) idx' (Some (k', w'))) in Hkvs_uniqueness; last by simplify_map_eq.
+    rewrite -insert_delete_eq in Hkvs_uniqueness.
+    rewrite kvs_keys_insert_Some in Hkvs_uniqueness; last by simplify_map_eq.
+    apply NoDup_cons in Hkvs_uniqueness as [Hk _ ].
+    apply not_elem_of_cons in Hk as [ HK _ ].
+    done.
+  Qed.
+
+  Lemma kvs_physical_map_open_diff
+    (a : Addr) (pkvs : kvs_physical_map) (idx idx' : nat) (k : full_key_t) (w : Word):
+    pkvs !! idx = Some (Some (k, w)) ->
+    0 <= idx' < SIZE_MAP ->
+    idx ≠ idx' ->
+    is_physical_kvs a pkvs -∗
+    ∃ opt_kw',
+      is_physical_kvs_open a pkvs idx' ∗
+      ⌜ pkvs !! idx' = Some opt_kw' ⌝ ∗
+      physical_kvs_entry a idx' opt_kw' ∗
+      ⌜ match opt_kw' with | Some kw' => k ≠ kw'.1 | None => True end ⌝.
+  Proof.
+    iIntros (Hpkvs_idx Hidx' Hidx_ne) "[%Hwf_kvs HKVS]".
+    pose proof (wf_kvs_is_Some _ _ Hwf_kvs Hidx') as [ opt_kw' Hm_idx' ].
+    iExists opt_kw'.
+    rewrite -{1}(insert_id pkvs idx' opt_kw'); last done.
+    iDestruct (big_sepM_insert_delete with "HKVS") as "[ Hk' HKVS]".
+    iFrame "∗%".
+    iPureIntro.
+    destruct opt_kw' as [ [k' w'] |]; auto.
+    pose proof (wf_kvs_neq _ _ _ _ _ _ _ Hwf_kvs Hidx_ne Hpkvs_idx Hm_idx') as Hkk'.
+    done.
+  Qed.
+
+
+  Lemma kvs_physical_map_close
+    (a : Addr) (pkvs : kvs_physical_map) (idx : nat) (opt_kwidx : kvs_physical_entry):
+    pkvs !! idx = Some opt_kwidx ->
+
+    is_physical_kvs_open a pkvs idx -∗
+    physical_kvs_entry a idx opt_kwidx -∗
+    is_physical_kvs a pkvs.
+  Proof.
+    iIntros (Hidx) "[%Hwf_kvs HKVS] Hentry"; cbn.
+    iDestruct (big_sepM_delete with "[$HKVS $Hentry]") as "HKVS"; eauto.
+    iFrame; eauto.
+  Qed.
+
+  Lemma kvs_keys_empty : kvs_keys ∅ = [].
+  Proof. rewrite /kvs_keys map_fold_empty; done. Qed.
+
+  Definition kvs_elem_of_kvs (pkvs : kvs_physical_map) (k : full_key_t) ( w : Word ) :=
+    (∃ idx, pkvs !! idx = Some (Some (k, w))).
+  Lemma elem_of_kvs_keys_1 (pkvs : kvs_physical_map) (k : full_key_t) :
+    k ∈ kvs_keys pkvs -> (∃ w, kvs_elem_of_kvs pkvs k w).
+  Proof.
+    move: k.
+    induction pkvs using map_ind ; intros k Hk.
+    { rewrite kvs_keys_empty in Hk; set_solver+Hk. }
+    destruct x as [ [k' w'] |].
+    - rewrite kvs_keys_insert_Some in Hk; auto.
+      apply elem_of_cons in Hk as [ -> | Hk].
+      + exists w', i ; simplify_map_eq; done.
+      + apply IHpkvs in Hk.
+        destruct Hk as (w & idx & Hidx).
+        exists w, idx.
+        assert (i ≠ idx) by (intro; simplify_map_eq;done).
+        simplify_map_eq; done.
+    - rewrite kvs_keys_insert_None in Hk; auto.
+      apply IHpkvs in Hk.
+      destruct Hk as (w & idx & Hidx).
+      exists w, idx.
+      assert (i ≠ idx) by (intro; simplify_map_eq;done).
+      simplify_map_eq; done.
+  Qed.
+
+  Lemma elem_of_kvs_keys_2 (pkvs : kvs_physical_map) (k : full_key_t) :
+    (∃ w, kvs_elem_of_kvs pkvs k w) ->
+    k ∈ kvs_keys pkvs.
+  Proof.
+    intros (w & idx & Hidx).
+    rewrite -(insert_id pkvs idx (Some (k, w))); last done.
+    rewrite -insert_delete_eq.
+    rewrite kvs_keys_insert_Some; last by simplify_map_eq.
+    apply elem_of_cons; by left.
+  Qed.
+
+  Lemma elem_of_kvs_keys (pkvs : kvs_physical_map) (k : full_key_t) :
+    k ∈ kvs_keys pkvs ↔ (∃ w, kvs_elem_of_kvs pkvs k w).
+  Proof. split ; [apply elem_of_kvs_keys_1 | apply elem_of_kvs_keys_2]. Qed.
+
+  Lemma kvs_physical_map_open_notin
+    (a : Addr) (pkvs : kvs_physical_map)
+    (idx : nat) (uk : user_key_t) (mk : map_key_t) :
+    let fkey := kvs_full_key uk mk in
+    is_uint16 mk ->
+    (0 ≤ idx < SIZE_MAP)%Z →
+    fkey ∉ kvs_keys pkvs ->
+    is_physical_kvs a pkvs -∗
+    ∃ opt_kwidx,
+      ⌜ pkvs !! idx = Some opt_kwidx ⌝ ∗
+      is_physical_kvs_open a pkvs idx ∗
+      physical_kvs_entry a idx opt_kwidx ∗
+      ⌜ match opt_kwidx with | Some kwidx => kwidx.1 ≠ fkey | None => True end ⌝.
+  Proof.
+    intros fkey Hwf_full_key Hidx Hs'.
+    iIntros "[%Hwf_kvs HKVS]".
+    assert ( is_Some (pkvs !! idx) ) as [ opt_kwidx Hm_idx].
+    { apply wf_kvs_is_Some; auto; lia. }
+    rewrite -{1}(insert_id pkvs idx opt_kwidx); last done.
+    iDestruct (big_sepM_insert_delete with "HKVS") as "[Hkvs_entry HKVS]".
+    iFrame "∗%".
+    iPureIntro.
+    destruct opt_kwidx as [ [ kidx widx ]|]; auto.
+    cbn.
+    assert ( kidx ∈ kvs_keys pkvs ) as Hkidx; last set_solver.
+    apply elem_of_kvs_keys; eexists _,_; eauto.
+  Qed.
+
+
+End KVS_physical_map.
+
+
+Definition kvs_user_map : Type := gmap map_key_t Word.
+Definition kvs_logical_map : Type := gmap user_key_t kvs_user_map.
+
+(* CMRA for KVS *)
+Class kvsG Σ :=
+  KvsG {
+      (* kvs_genG :: gen_heapGS nat kvs_entry Σ; *)
+      kvs_logical_genG :: gen_heapGS user_key_t kvs_user_map Σ;
+    }.
+
+Notation "'↪●LKVS' lkvs" :=
+  ( gen_heap_interp (L:=user_key_t) (V:= kvs_user_map) lkvs )%I (at level 20) : bi_scope.
+Notation "uk '↦(LKVS)[' dq ']' m" :=
+  (pointsto (L:=user_key_t) (V:= kvs_user_map) uk dq m)%I (at level 20) : bi_scope.
+Notation "uk '↦(LKVS)' m" :=
+  (uk ↦(LKVS)[ (DfracOwn 1) ] m)%I (at level 20) : bi_scope.
+
+Lemma kvs_logical_kvs_valid `{kvsG}
+  (uk : user_key_t) (lkvs : kvs_logical_map) (m : kvs_user_map) :
+  ↪●LKVS lkvs  -∗ uk ↦(LKVS) m -∗ ⌜ lkvs !! uk = Some m ⌝.
+Proof.
+  iIntros "Hauth Hfrag".
+  by iDestruct (gen_heap_valid with "Hauth Hfrag") as "%Hvalid".
+Qed.
+
+Lemma kvs_logical_kvs_update `{kvsG}
+  (uk : user_key_t) (lkvs : kvs_logical_map) (m m' : kvs_user_map) :
+  ↪●LKVS lkvs -∗ uk ↦(LKVS) m
+  ==∗
+  ↪●LKVS (<[uk := m']> lkvs) ∗ uk ↦(LKVS) m'.
+Proof.
+  iIntros "Hauth Hfrag".
+  by iMod (gen_heap_update lkvs uk _ m' with "Hauth Hfrag") as "[$ $]".
+Qed.
+
+
+Class kvs_namespaces :=
+  {
+    Nkvs : namespace;
+    Nkvs_otype : namespace;
+    Nkvs_exp_tbl : namespace;
+    Nkvs_namespaces_disjoint :
+    Nkvs ## Nkvs_otype ∧ Nkvs ## Nkvs_exp_tbl ∧ Nkvs_otype ## Nkvs_exp_tbl
+  }.
+
+
+Section KVS_logical_map.
+  Context
+    {Σ:gFunctors}
+    {ceriseg:ceriseG Σ}
+    {kvsg:kvsG Σ}
+    `{MP: MachineParameters}
+  .
+
+
+  Definition kvs_elem_of_logical_kvs
+    (lkvs : kvs_logical_map) (uk : user_key_t) (mk : map_key_t) ( w : Word ) :=
+    (∃ ukvs, lkvs !! uk = Some ukvs ∧  ukvs !! mk = Some w).
+
+  Definition kvs_synced_logical_kvs (pkvs : kvs_physical_map) (lkvs : kvs_logical_map) : Prop :=
+    ∀ (k : user_key_t * map_key_t) (w : Word),
+    is_uint16 k.2 ->
+    ( kvs_elem_of_logical_kvs lkvs k.1 k.2 w ↔ kvs_elem_of_kvs pkvs (kvs_full_key k.1 k.2) w).
+
+  Definition is_logical_kvs (a : Addr) (lkvs : kvs_logical_map) : iProp Σ :=
+    ∃ (pkvs : kvs_physical_map),
+      ⌜ kvs_synced_logical_kvs pkvs lkvs ⌝ ∗ is_physical_kvs a pkvs.
+
+  Definition logical_kvs_inv (a : Addr) : iProp Σ :=
+      ∃ (lkvs : kvs_logical_map), ↪●LKVS lkvs ∗ (is_logical_kvs a lkvs).
+
+
+  Lemma kvs_synced_logical_lookup_Some
+    (pkvs : kvs_physical_map) (lkvs : kvs_logical_map) (m : kvs_user_map)
+    (uk : user_key_t) (mk : map_key_t) (w : Word) :
+    let fkey := kvs_full_key uk mk in
+    is_uint16 mk ->
+    kvs_synced_logical_kvs pkvs lkvs ->
+    lkvs !! uk = Some m ->
+    m !! mk = Some w ->
+    ∃ idx, pkvs !! idx = Some (Some (fkey, w)).
+  Proof.
+    rewrite /kvs_synced_logical_kvs.
+    intros Huint16_mk Hsync Hlkvs_uk Hm_mk.
+    specialize (Hsync (uk,mk) w Huint16_mk); cbn in *.
+    apply Hsync.
+    eexists; split; eauto.
+  Qed.
+
+  Lemma kvs_synced_logical_lookup_None
+    (pkvs : kvs_physical_map) (lkvs : kvs_logical_map) (m : kvs_user_map)
+    (uk : user_key_t) (mk : map_key_t) :
+    let fkey := kvs_full_key uk mk in
+    is_uint16 mk ->
+    kvs_synced_logical_kvs pkvs lkvs ->
+    lkvs !! uk = Some m ->
+    m !! mk = None ->
+    fkey ∉ kvs_keys pkvs.
+  Proof.
+    rewrite /kvs_synced_logical_kvs.
+    intros Huint16_mk Hsync Hlkvs_uk Hm_mk.
+    intros Hcontra.
+    apply elem_of_kvs_keys in Hcontra as (w & Hcontra).
+    specialize (Hsync (uk,mk) w Huint16_mk); cbn in *.
+    apply Hsync in Hcontra as (m'&Hm'&Hcontra); simplify_map_eq.
+  Qed.
+
+End KVS_logical_map.
+
+
+(* Section KVS_user_map. *)
+(*   Context *)
+(*     {Σ:gFunctors} *)
+(*     {ceriseg:ceriseG Σ} *)
+(*     {kvsg:kvsG Σ} *)
+(*     `{MP: MachineParameters} *)
+(*   . *)
+
+(*   Definition is_user_kvs `{kvs_namespaces} (a : Addr) (uk : user_key_t) (m : kvs_user_map) : iProp Σ := *)
+(*     logical_kvs_inv a ∗ uk ↦(LKVS) m. *)
+
+(*   Definition kvs_user_pointsto (uk : user_key_t) (mk : map_key_t) (w : Word) := *)
+(*     (uk,mk) ↦(UKVS) w *)
+
+
+
+
+(* End KVS_user_map. *)
+
+(*     ●(KVS) m ∗ *)
+(*     ↪●KVS_USERS lm ∗ *)
+
+
+
+
+
+
+
+
+(* Definition kvs_frag_idx_frac `{kvsG} (idx : nat) (k : Z) (w : Word) (q : dfrac) : iProp Σ := *)
+(*   (pointsto (L:=nat) (V:=kvs_entry) idx q (Some (k,w))). *)
+(* Notation "k '⤇(KVS){' q '}[' idx  ']' w" := *)
+(*   (kvs_frag_idx_frac idx k w q) (at level 20) : bi_scope. *)
+(* Notation "k '⤇(KVS){' q '}[' idx  ']' -" := *)
+(*   (∃ w, kvs_frag_idx_frac idx k w q)%I (at level 20) : bi_scope. *)
+
+(* Notation "idx '⤇(KVS)' 'NONE'" := *)
+(*   (pointsto (L:=nat) (V:=kvs_entry) idx (DfracOwn 1) None) (at level 20) : bi_scope. *)
+(* Notation "k '⤇(KVS)[' idx  ']' w" := *)
+(*   (kvs_frag_idx_frac idx k w (DfracOwn 1)) (at level 20) : bi_scope. *)
+(* Notation "k '⤇(KVS)[' idx  ']' -" := *)
+(*   (∃ w, kvs_frag_idx_frac idx k w (DfracOwn 1))%I (at level 20) : bi_scope. *)
+
+(* Definition kvs_frag `{kvsG} (k : Z ) (w : Word) : iProp Σ := ∃ idx, k ⤇(KVS)[ idx ] w. *)
+(* Notation "k '⤇(KVS)' w" := (kvs_frag k w) (at level 20) : bi_scope. *)
+(* Notation "k '⤇(KVS)' -" := (∃ w, kvs_frag k w)%I (at level 20) : bi_scope. *)
+
+(* Notation "●(KVS) m" := (gen_heap_interp (m : kvs_map)) (at level 20) : bi_scope. *)
+
+Section KVS_preamble.
+  Context
+    {Σ:gFunctors}
+    {ceriseg:ceriseG Σ}
+    {kvsg:kvsG Σ}
+    `{MP: MachineParameters}
+  .
+
 
   Local Lemma kvs_not_elem_of_logical_kvs (lm : kvs_logical_map) (uk mk : Z) ( w : Word ) :
     ¬ kvs_elem_of_logical_kvs lm uk mk w ->
@@ -218,6 +568,9 @@ Section KVS_preamble.
   Definition kvs_logical_kvs_insert (lm : kvs_logical_map) (uk mk : Z) (w : Word) :=
    <[uk := (<[ mk := w ]> (default ∅ (lm !! uk))) ]> lm.
 
+  Definition kvs_logical_kvs_delete (lm : kvs_logical_map) (uk mk : Z) :=
+   <[uk := (delete mk (default ∅ (lm !! uk))) ]> lm.
+
   Lemma kvs_logical_kvs_insert_lookup_eq (lm : kvs_logical_map) (uk mk : Z) (w : Word) (umap : kvs_user_map) :
     kvs_logical_kvs_insert lm uk mk w !! uk = Some umap ->
     umap = <[mk := w]> (default ∅ (lm !! uk)).
@@ -236,9 +589,6 @@ Section KVS_preamble.
     rewrite /kvs_logical_kvs_insert in H; simplify_map_eq.
     done.
   Qed.
-
-  Definition kvs_logical_kvs_delete (lm : kvs_logical_map) (uk mk : Z) :=
-   <[uk := (delete mk (default ∅ (lm !! uk))) ]> lm.
 
   Lemma kvs_logical_kvs_delete_lookup_eq
     (lm : kvs_logical_map) (uk mk : Z) (umap : kvs_user_map) :
@@ -261,154 +611,24 @@ Section KVS_preamble.
     done.
   Qed.
 
-  Definition kvs_elem_of_kvs (mkvs : kvs_map) (k : Z) ( w : Word ) :=
-    (∃ idx, mkvs !! idx = Some (Some (k, w))).
+  (* Definition isKVS *)
+  (*   (a : Addr) (m : kvs_map) (lm : kvs_logical_map) : iProp Σ := *)
+  (*   ⌜ wf_kvs_map m ⌝ ∗ *)
+  (*   ⌜ kvs_synced_logical_kvs m lm ⌝ ∗ *)
+  (*   ●(KVS) m ∗ *)
+  (*   ↪●KVS_USERS lm ∗ *)
+  (*   [∗ map] idx ↦ kw ∈ m, isKVS_entry a idx kw. *)
 
-  Definition kvs_synced_logical_kvs (m : kvs_map) (lm : kvs_logical_map) : Prop :=
-    ∀ k w, is_uint16 k.2 ->
-         ( kvs_elem_of_logical_kvs lm k.1 k.2 w ↔ kvs_elem_of_kvs m (kvs_full_key k.1 k.2) w).
-
-  Definition isKVS
-    (a : Addr) (m : kvs_map) (lm : kvs_logical_map) : iProp Σ :=
-    ⌜ wf_kvs_map m ⌝ ∗
-    ⌜ kvs_synced_logical_kvs m lm ⌝ ∗
-    ●(KVS) m ∗
-    ↪●KVS_USERS lm ∗
-    [∗ map] idx ↦ kw ∈ m, isKVS_entry a idx kw.
-
-  Definition isKVS_open
-    (a : Addr) (m : kvs_map) (lm : kvs_logical_map) (open_idx : nat) : iProp Σ :=
-    ⌜ wf_kvs_map m ⌝ ∗
-    ⌜ kvs_synced_logical_kvs m lm ⌝ ∗
-    ●(KVS) m ∗
-    ↪●KVS_USERS lm ∗
-    [∗ map] idx ↦ kw ∈ (delete open_idx m), isKVS_entry a idx kw.
-
-  Lemma wf_kvs_is_Some (m : kvs_map) (idx : nat)  :
-    wf_kvs_map m ->
-    0 <= idx < SIZE_MAP ->
-    is_Some (m !! idx).
-  Proof.
-    intros [Hkvs_dom _] Hidx.
-    apply elem_of_dom.
-    rewrite Hkvs_dom /kvs_dom.
-    by apply elem_of_set_seq.
-  Qed.
-
-  Lemma wf_kvs_indom_idx (m : kvs_map) (idx : nat) :
-    idx ∈ dom m ->
-    wf_kvs_map m ->
-    0 <= idx < SIZE_MAP.
-  Proof.
-    intros Hm_idx [Hkvs_dom _].
-    rewrite Hkvs_dom /kvs_dom in Hm_idx.
-    apply elem_of_set_seq in Hm_idx.
-    lia.
-  Qed.
-
-  Global Instance Permutation_Reflexive {A} : Reflexive (@Permutation A).
-  Proof. intros l ; done. Qed.
-
-  Global Instance Permutation_Transitive {A} : Transitive (@Permutation A).
-  Proof. intros l1 l2 l3 Hl12 Hl23; eapply Permutation_trans; done. Qed.
-
-  Global Instance Permutation_PreOrder {A} : PreOrder (@Permutation A).
-  Proof. split; apply _. Qed.
-
-  Local Instance Proper_get_kvs_key (opt_kv : kvs_entry) :
-  Proper (Permutation ==> Permutation)
-    (λ acc : list Z, match opt_kv with
-                     | Some kv => kv.1 :: acc
-                     | None => acc
-                     end).
-  Proof. intros l1 l2 Hl; destruct opt_kv; auto. Qed.
-
-  Lemma kvs_keys_insert_None idx m :
-    m !! idx = None ->
-    kvs_keys (<[idx:=None]> m) ≡ₚ kvs_keys m.
-  Proof.
-    intros Hidx.
-    rewrite /kvs_keys.
-    setoid_rewrite map_fold_insert; auto; try apply _.
-    intros j1 j2 opt_kv1 opt_kv2 l Hk_neq Hj1 Hj2.
-    destruct opt_kv1, opt_kv2; auto.
-    econstructor.
-  Qed.
+  (* Definition isKVS_open *)
+  (*   (a : Addr) (m : kvs_map) (lm : kvs_logical_map) (open_idx : nat) : iProp Σ := *)
+  (*   ⌜ wf_kvs_map m ⌝ ∗ *)
+  (*   ⌜ kvs_synced_logical_kvs m lm ⌝ ∗ *)
+  (*   ●(KVS) m ∗ *)
+  (*   ↪●KVS_USERS lm ∗ *)
+  (*   [∗ map] idx ↦ kw ∈ (delete open_idx m), isKVS_entry a idx kw. *)
 
 
-  Lemma kvs_keys_insert_Some idx k w m :
-    m !! idx = None ->
-    kvs_keys (<[idx:=Some (k, w)]> m) ≡ₚ (k :: kvs_keys m).
-  Proof.
-    intros Hidx.
-    rewrite /kvs_keys.
-    setoid_rewrite map_fold_insert; auto; try apply _.
-    intros j1 j2 opt_kv1 opt_kv2 l Hk_neq Hj1 Hj2.
-    destruct opt_kv1, opt_kv2; auto.
-    econstructor.
-  Qed.
-
-  Lemma wf_kvs_neq (m : kvs_map) (idx idx' : nat) (k k' : Z) (w w' : Word) :
-    wf_kvs_map m ->
-    idx ≠ idx' ->
-    m !! idx = Some (Some (k, w)) ->
-    m !! idx' = Some (Some (k', w')) ->
-    k ≠ k'.
-  Proof.
-    intros [_ Hkvs_uniqueness] Hidx_ne Hm_idx Hm_idx'.
-    rewrite -(insert_id m idx (Some (k, w))) in Hkvs_uniqueness; last done.
-    rewrite -insert_delete_eq in Hkvs_uniqueness.
-    rewrite kvs_keys_insert_Some in Hkvs_uniqueness; last by simplify_map_eq.
-    rewrite -(insert_id (delete idx m) idx' (Some (k', w'))) in Hkvs_uniqueness; last by simplify_map_eq.
-    rewrite -insert_delete_eq in Hkvs_uniqueness.
-    rewrite kvs_keys_insert_Some in Hkvs_uniqueness; last by simplify_map_eq.
-    apply NoDup_cons in Hkvs_uniqueness as [Hk _ ].
-    apply not_elem_of_cons in Hk as [ HK _ ].
-    done.
-  Qed.
-
-  Lemma kvs_keys_empty : kvs_keys ∅ = [].
-  Proof. rewrite /kvs_keys map_fold_empty; done. Qed.
-
-  Lemma elem_of_kvs_keys_1 (m : kvs_map) (k : Z) :
-    k ∈ kvs_keys m -> (∃ idx w, m !! idx = Some (Some (k, w))).
-  Proof.
-    move: k.
-    induction m using map_ind ; intros k Hk.
-    { rewrite kvs_keys_empty in Hk; set_solver+Hk. }
-    destruct x as [ [k' w'] |].
-    - rewrite kvs_keys_insert_Some in Hk; auto.
-      apply elem_of_cons in Hk as [ -> | Hk].
-      + exists i, w' ; simplify_map_eq; done.
-      + apply IHm in Hk.
-        destruct Hk as (idx & w & Hidx).
-        exists idx, w.
-        assert (i ≠ idx) by (intro; simplify_map_eq;done).
-        simplify_map_eq; done.
-    - rewrite kvs_keys_insert_None in Hk; auto.
-      apply IHm in Hk.
-      destruct Hk as (idx & w & Hidx).
-      exists idx, w.
-      assert (i ≠ idx) by (intro; simplify_map_eq;done).
-      simplify_map_eq; done.
-  Qed.
-
-  Lemma elem_of_kvs_keys_2 (m : kvs_map) (k : Z) :
-    (∃ idx w, m !! idx = Some (Some (k, w))) ->
-    k ∈ kvs_keys m.
-  Proof.
-    intros (idx & w & Hidx).
-    rewrite -(insert_id m idx (Some (k, w))); last done.
-    rewrite -insert_delete_eq.
-    rewrite kvs_keys_insert_Some; last by simplify_map_eq.
-    apply elem_of_cons; by left.
-  Qed.
-
-  Lemma elem_of_kvs_keys (m : kvs_map) (k : Z) :
-    k ∈ kvs_keys m ↔ (∃ idx w, m !! idx = Some (Some (k, w))).
-  Proof. split ; [apply elem_of_kvs_keys_1 | apply elem_of_kvs_keys_2]. Qed.
-
-  Lemma NoDup_kvs_keys_update (m : kvs_map) (idx : nat) (k : Z) (w w' : Word) :
+  Lemma NoDup_kvs_keys_update (m : kvs_physical_map) (idx : nat) (k : Z) (w w' : Word) :
     m !! idx = Some (Some (k, w)) ->
     NoDup (kvs_keys m) ->
     NoDup (kvs_keys (<[idx := Some (k, w') ]>m)).
@@ -426,19 +646,19 @@ Section KVS_preamble.
         apply NoDup_cons in Hnodup as [HkX Hnodup].
         apply NoDup_cons; split; last (eapply IHm; eauto).
         intro Hcontra.
-        apply elem_of_kvs_keys in Hcontra as (idx0 & w0 & H0).
+        apply elem_of_kvs_keys in Hcontra as (w0 & idx0 & H0).
         apply HkX.
         apply elem_of_kvs_keys; auto.
         destruct (decide (idx = idx0)); simplify_map_eq.
-        { exists idx0, w; done. }
-        { exists idx0, w0; done. }
+        { exists w, idx0; done. }
+        { exists w0, idx0; done. }
       + rewrite kvs_keys_insert_None in Hnodup; auto.
         rewrite kvs_keys_insert_None; simplify_map_eq; auto.
         eapply IHm; eauto.
   Qed.
 
   Lemma NoDup_kvs_keys_insert_Some
-    (m : kvs_map) (idx : nat) (k : Z) (w : Word) :
+    (m : kvs_physical_map) (idx : nat) (k : Z) (w : Word) :
     k ∉ kvs_keys m ->
     NoDup (kvs_keys m) ->
     NoDup (kvs_keys (<[idx:= Some (k, w)]> m)).
@@ -471,7 +691,7 @@ Section KVS_preamble.
         apply NoDup_cons; split; auto.
         intro Hcontra.
         apply elem_of_kvs_keys in Hcontra.
-        destruct Hcontra as (idx0&w0&Hcontra).
+        destruct Hcontra as (w0&idx0&Hcontra).
         destruct (decide (idx0 = idx)); simplify_map_eq.
         apply Hk'.
         apply elem_of_kvs_keys.
@@ -482,7 +702,7 @@ Section KVS_preamble.
   Qed.
 
   Lemma NoDup_kvs_keys_insert_None
-    (m : kvs_map) (idx : nat) :
+    (m : kvs_physical_map) (idx : nat) :
     m !! idx = None ->
     NoDup (kvs_keys m) ->
     NoDup (kvs_keys (<[idx:= None]> m)).
@@ -491,12 +711,12 @@ Section KVS_preamble.
     rewrite kvs_keys_insert_None; auto.
   Qed.
 
-  Definition kvs_map_init : kvs_map :=
+  Definition kvs_physical_map_init : kvs_physical_map :=
     list_to_map ((fun n => (n, None)) <$> (seq 0 SIZE_MAP)).
 
-  Lemma wf_kvs_map_kvs_map_init : wf_kvs_map kvs_map_init.
+  Lemma wf_kvs_physical_map_kvs_physical_map_init : wf_kvs_physical_map kvs_physical_map_init.
   Proof.
-    rewrite /kvs_map_init /wf_kvs_map /kvs_dom.
+    rewrite /kvs_physical_map_init /wf_kvs_physical_map /kvs_dom.
     generalize 0 as k.
     induction SIZE_MAP; intros k; cbn.
     - split.
@@ -517,9 +737,9 @@ Section KVS_preamble.
         lia.
   Qed.
 
-  Lemma kvs_keys_map_init : kvs_keys kvs_map_init ≡ₚ [].
+  Lemma kvs_keys_map_init : kvs_keys kvs_physical_map_init ≡ₚ [].
   Proof.
-    rewrite /kvs_map_init.
+    rewrite /kvs_physical_map_init.
     generalize 0 as k.
     induction SIZE_MAP; intros k; cbn.
     - by rewrite kvs_keys_empty.
@@ -533,8 +753,8 @@ Section KVS_preamble.
       lia.
   Qed.
 
-  Lemma kvs_not_elem_of_kvs_map_init_lookup k w :
-    ¬ (kvs_elem_of_kvs kvs_map_init k w).
+  Lemma kvs_not_elem_of_kvs_physical_map_init_lookup k w :
+    ¬ (kvs_elem_of_kvs kvs_physical_map_init k w).
   Proof.
     intros Hkvs.
     cbn in Hkvs.
@@ -545,58 +765,58 @@ Section KVS_preamble.
 
   Lemma kvs_alloc_synced_map_init (m : kvs_logical_map) :
     (∀ ku sk, m !! ku = Some sk -> sk = ∅) ->
-    kvs_synced_logical_kvs kvs_map_init m.
+    kvs_synced_logical_kvs kvs_physical_map_init m.
   Proof.
     intros Hm.
     intros [ku kn] w Hwf_k; cbn in *.
     split; intros Hkvs; exfalso.
     - destruct Hkvs as (sk & Hk & Hsk).
       apply Hm in Hk; set_solver.
-    - eapply kvs_not_elem_of_kvs_map_init_lookup; eauto.
+    - eapply kvs_not_elem_of_kvs_physical_map_init_lookup; eauto.
   Qed.
 
-  Lemma elem_of_kvs_map_init (idx : nat) (opt_kv : kvs_entry) :
-    kvs_map_init !! idx = Some opt_kv -> opt_kv = None.
+  Lemma elem_of_kvs_physical_map_init (idx : nat) (opt_kv : kvs_physical_entry) :
+    kvs_physical_map_init !! idx = Some opt_kv -> opt_kv = None.
   Proof.
     intros Hidx.
-    rewrite /kvs_map_init in Hidx.
+    rewrite /kvs_physical_map_init in Hidx.
     apply elem_of_list_to_map_2 in Hidx.
     apply list_elem_of_fmap in Hidx as (n&?&Hidx); simplify_eq.
     done.
   Qed.
 
-  Lemma kvs_initial_map_init_None :
-  ([∗ map] l↦v ∈ kvs_map_init, pointsto l (DfracOwn 1) v) -∗
-  ([∗ map] idx↦_ ∈ kvs_map_init, idx⤇(KVS) NONE).
-  Proof.
-    iIntros "Hkvs_frags".
-    iApply (big_sepM_impl with "Hkvs_frags").
-    iModIntro; iIntros (k v Hk) "H".
-    apply elem_of_kvs_map_init in Hk; simplify_eq; iFrame.
-  Qed.
+  (* Lemma kvs_initial_map_init_None : *)
+  (* ([∗ map] l↦v ∈ kvs_physical_map_init, pointsto l (DfracOwn 1) v) -∗ *)
+  (* ([∗ map] idx↦_ ∈ kvs_physical_map_init, idx⤇(KVS) NONE). *)
+  (* Proof. *)
+  (*   iIntros "Hkvs_frags". *)
+  (*   iApply (big_sepM_impl with "Hkvs_frags"). *)
+  (*   iModIntro; iIntros (k v Hk) "H". *)
+  (*   apply elem_of_kvs_physical_map_init in Hk; simplify_eq; iFrame. *)
+  (* Qed. *)
 
   Lemma kvs_initial_map_init (b e : Addr) :
     (b + (ASM_SIZEOF_KVS_ENTRY * SIZE_MAP))%a = Some e ->
     ([[b,e]]↦ₐ[[kvs_data]]) -∗
-    ([∗ map] idx↦opt_kw ∈ kvs_map_init, idx ⤇(KVS) NONE) -∗
-    [∗ map] idx↦kw ∈ kvs_map_init, isKVS_entry b idx kw.
+    (* ([∗ map] idx↦opt_kw ∈ kvs_physical_map_init, idx ⤇(KVS) NONE) -∗ *)
+    [∗ map] idx↦kw ∈ kvs_physical_map_init, physical_kvs_entry b idx kw.
   Proof.
-    rewrite /kvs_map_init /kvs_data.
+    rewrite /kvs_physical_map_init /kvs_data.
     generalize dependent e.
     replace b with (b^+(ASM_SIZEOF_KVS_ENTRY*0%nat))%a by solve_addr.
     rewrite {3}(_ : (b^+(ASM_SIZEOF_KVS_ENTRY*0%nat))%a = b); last solve_addr.
     generalize 0 as k.
-    induction SIZE_MAP; iIntros (k e Hbe) "Hmem Hfrags"; cbn; first done.
+    induction SIZE_MAP; iIntros (k e Hbe) "Hmem"; cbn; first done.
 
     specialize (IHn (S k)).
-    iDestruct (big_sepM_insert with "Hfrags") as "[Hf Hfrags]".
-    { apply not_elem_of_list_to_map.
-      intro Hcontra.
-      apply list_elem_of_fmap in Hcontra as ([idx opt_kw ] & ? & Hcontra); simplify_eq.
-      apply list_elem_of_fmap in Hcontra as (k' & ? & Hcontra); simplify_eq.
-      apply elem_of_seq in Hcontra; cbn in *.
-      lia.
-    }
+    (* iDestruct (big_sepM_insert with "Hfrags") as "[Hf Hfrags]". *)
+    (* { apply not_elem_of_list_to_map. *)
+    (*   intro Hcontra. *)
+    (*   apply list_elem_of_fmap in Hcontra as ([idx opt_kw ] & ? & Hcontra); simplify_eq. *)
+    (*   apply list_elem_of_fmap in Hcontra as (k' & ? & Hcontra); simplify_eq. *)
+    (*   apply elem_of_seq in Hcontra; cbn in *. *)
+    (*   lia. *)
+    (* } *)
     iApply big_sepM_insert.
     { apply not_elem_of_list_to_map.
       intro Hcontra.
@@ -617,19 +837,19 @@ Section KVS_preamble.
                  with "Hmem") as "[Hasm_idx Hmem]"
     ; [ solve_addr+Hbe | symmetry; apply finz_incr_iff_dist; solve_addr+Hbe | ].
 
-    iSplitL "Hf Hasm_idx".
+    iSplitL "Hasm_idx".
     - iFrame.
-    - iApply (IHn (b ^+ (ASM_SIZEOF_KVS_ENTRY * (k + (S n))))%a with "[Hmem] [$Hfrags]"); first solve_addr+Hbe.
+    - iApply (IHn (b ^+ (ASM_SIZEOF_KVS_ENTRY * (k + (S n))))%a with "[Hmem]"); first solve_addr+Hbe.
       replace (b ^+ ASM_SIZEOF_KVS_ENTRY * S k)%a with (b ^+ (ASM_SIZEOF_KVS_ENTRY * k + ASM_SIZEOF_KVS_ENTRY))%a by solve_addr.
       replace e with (b ^+ ASM_SIZEOF_KVS_ENTRY * (k + S n))%a by solve_addr.
       done.
   Qed.
 
-  Lemma wf_kvs_map_insert (m : kvs_map) (idx : nat) (k : Z) (w : Word) :
+  Lemma wf_kvs_physical_map_insert (m : kvs_physical_map) (idx : nat) (k : Z) (w : Word) :
     m !! idx = Some None ->
     k ∉ kvs_keys m ->
-    wf_kvs_map m ->
-    wf_kvs_map (<[idx:= Some (k, w)]> m).
+    wf_kvs_physical_map m ->
+    wf_kvs_physical_map (<[idx:= Some (k, w)]> m).
   Proof.
     intros Hidx Hk (Hkvs_dom & Hkvs_unique).
     split.
@@ -641,7 +861,7 @@ Section KVS_preamble.
   Qed.
 
   Local Lemma kvs_synced_logical_kvs_insert_1
-    (m : kvs_map) ( lm : kvs_logical_map )
+    (m : kvs_physical_map) ( lm : kvs_logical_map )
     (idx : nat)
     (uk mk uk' mk' : Z) (w w' : Word) :
     let fkey := kvs_full_key uk mk in
@@ -660,8 +880,9 @@ Section KVS_preamble.
       + eexists idx; simplify_map_eq; done.
       + specialize (Halloc (uk', mk') w' Hwf_full_key'); cbn in *.
         rewrite /kvs_elem_of_logical_kvs in Halloc.
-        destruct ( lm !! uk' ) as [umap_uk|]; last set_solver+Hmk'.
+        destruct ( lm !! uk' ) as [umap_uk|] eqn:Hlm; last set_solver+Hmk'.
         cbn in Hmk'.
+        rewrite Hlm in Halloc.
         assert (∃ umap : kvs_user_map, Some umap_uk = Some umap
                                        ∧ umap !! mk' = Some w') as IH.
         { exists umap_uk; split; auto. }
@@ -681,7 +902,7 @@ Section KVS_preamble.
   Qed.
 
   Local Lemma kvs_synced_logical_kvs_insert_2
-    (m : kvs_map) ( lm : kvs_logical_map )
+    (m : kvs_physical_map) ( lm : kvs_logical_map )
     (idx : nat)
     (uk mk uk' mk' : Z) (w w' : Word) :
     let fkey := kvs_full_key uk mk in
@@ -697,7 +918,7 @@ Section KVS_preamble.
     specialize (Halloc (uk', mk') w' Hwf_full_key') as IH.
     destruct Hk as (idx' & Hk).
     destruct (decide (idx = idx')); simplify_map_eq; cbn in *; auto.
-    - apply kvs_full_key_inj in H as [ -> -> ]; eauto.
+    - apply kvs_full_key_inj in Hk as [ -> -> ]; eauto.
       rewrite /kvs_logical_kvs_insert;simplify_map_eq.
       rewrite /kvs_elem_of_logical_kvs;simplify_map_eq.
       exists (<[mk':=w']> (default ∅ (lm !! uk'))); split; auto.
@@ -716,7 +937,7 @@ Section KVS_preamble.
         eexists ; split; eauto.
   Qed.
 
-  Lemma kvs_synced_logical_kvs_insert (m : kvs_map) ( lm : kvs_logical_map ) (idx : nat) (uk mk : Z) (w : Word) :
+  Lemma kvs_synced_logical_kvs_insert (m : kvs_physical_map) ( lm : kvs_logical_map ) (idx : nat) (uk mk : Z) (w : Word) :
     let fkey := kvs_full_key uk mk in
     is_uint16 mk ->
     m !! idx = Some None ->
@@ -732,10 +953,10 @@ Section KVS_preamble.
     - eapply kvs_synced_logical_kvs_insert_2; eauto.
   Qed.
 
-  Lemma wf_kvs_map_update (m : kvs_map) (idx : nat) (k : Z) (w : Word) :
+  Lemma wf_kvs_physical_map_update (m : kvs_physical_map) (idx : nat) (k : Z) (w : Word) :
     (∃ w', m !! idx = Some (Some (k, w'))) ->
-    wf_kvs_map m ->
-    wf_kvs_map (<[idx:= Some (k, w)]> m).
+    wf_kvs_physical_map m ->
+    wf_kvs_physical_map (<[idx:= Some (k, w)]> m).
   Proof.
     intros [w' Hidx] (Hkvs_dom & Hkvs_unique).
     split.
@@ -746,237 +967,237 @@ Section KVS_preamble.
     - eapply NoDup_kvs_keys_update; eauto.
   Qed.
 
-  Lemma kvs_frag_kvs_frag_idx (k : Z) (w : Word) :
-    k ⤇(KVS) w -∗ ∃ idx, k ⤇(KVS)[idx] w.
-  Proof. rewrite /kvs_frag; iIntros "?"; done. Qed.
+  (* Lemma kvs_frag_kvs_frag_idx (k : Z) (w : Word) : *)
+  (*   k ⤇(KVS) w -∗ ∃ idx, k ⤇(KVS)[idx] w. *)
+  (* Proof. rewrite /kvs_frag; iIntros "?"; done. Qed. *)
 
-  Lemma kvs_frag_idx_kvs_frag (k : Z) (w : Word) (idx : nat) :
-    k ⤇(KVS)[idx] w -∗ k ⤇(KVS) w.
-  Proof. rewrite /kvs_frag; iIntros "$".  Qed.
+  (* Lemma kvs_frag_idx_kvs_frag (k : Z) (w : Word) (idx : nat) : *)
+  (*   k ⤇(KVS)[idx] w -∗ k ⤇(KVS) w. *)
+  (* Proof. rewrite /kvs_frag; iIntros "$".  Qed. *)
 
-  Lemma kvs_auth_insert (a : Addr) (m : kvs_map) (idx : nat) (k : Z) (w : Word) :
-    ●(KVS) m -∗ idx ⤇(KVS) NONE
-    ==∗
-    ●(KVS) (<[idx:= Some (k, w)]> m) ∗ k ⤇(KVS)[ idx ] w.
-  Proof.
-    iIntros "Hkvs_auth Hkvs_frag".
-    by iMod (gen_heap_update m idx _ (Some (k,w)) with "Hkvs_auth Hkvs_frag") as "[$ $]".
-  Qed.
+  (* Lemma kvs_auth_insert (a : Addr) (m : kvs_physical_map) (idx : nat) (k : Z) (w : Word) : *)
+  (*   ●(KVS) m -∗ idx ⤇(KVS) NONE *)
+  (*   ==∗ *)
+  (*   ●(KVS) (<[idx:= Some (k, w)]> m) ∗ k ⤇(KVS)[ idx ] w. *)
+  (* Proof. *)
+  (*   iIntros "Hkvs_auth Hkvs_frag". *)
+  (*   by iMod (gen_heap_update m idx _ (Some (k,w)) with "Hkvs_auth Hkvs_frag") as "[$ $]". *)
+  (* Qed. *)
 
-  Lemma kvs_auth_update (a : Addr) (m : kvs_map) (idx : nat) (k k' : Z) (w w' : Word) :
-    ●(KVS) m -∗ k ⤇(KVS)[ idx ] w
-    ==∗
-    ●(KVS) (<[idx:= Some (k', w')]> m) ∗ k' ⤇(KVS)[ idx ] w'.
-  Proof.
-    iIntros "Hkvs_auth Hkvs_frag".
-    by iMod (gen_heap_update m idx _ (Some (k',w')) with "Hkvs_auth Hkvs_frag") as "[$ $]".
-  Qed.
+  (* Lemma kvs_auth_update (a : Addr) (m : kvs_physical_map) (idx : nat) (k k' : Z) (w w' : Word) : *)
+  (*   ●(KVS) m -∗ k ⤇(KVS)[ idx ] w *)
+  (*   ==∗ *)
+  (*   ●(KVS) (<[idx:= Some (k', w')]> m) ∗ k' ⤇(KVS)[ idx ] w'. *)
+  (* Proof. *)
+  (*   iIntros "Hkvs_auth Hkvs_frag". *)
+  (*   by iMod (gen_heap_update m idx _ (Some (k',w')) with "Hkvs_auth Hkvs_frag") as "[$ $]". *)
+  (* Qed. *)
 
-  Lemma kvs_auth_delete (a : Addr) (m : kvs_map) (idx : nat) (k : Z) (w : Word) :
-    ●(KVS) m -∗ k ⤇(KVS)[ idx ] w
-    ==∗
-    ●(KVS) (<[idx:= None]> m) ∗ idx ⤇(KVS) NONE.
-  Proof.
-    iIntros "Hkvs_auth Hkvs_frag".
-    by iMod (gen_heap_update m idx _ None with "Hkvs_auth Hkvs_frag") as "[$ $]".
-  Qed.
+  (* Lemma kvs_auth_delete (a : Addr) (m : kvs_physical_map) (idx : nat) (k : Z) (w : Word) : *)
+  (*   ●(KVS) m -∗ k ⤇(KVS)[ idx ] w *)
+  (*   ==∗ *)
+  (*   ●(KVS) (<[idx:= None]> m) ∗ idx ⤇(KVS) NONE. *)
+  (* Proof. *)
+  (*   iIntros "Hkvs_auth Hkvs_frag". *)
+  (*   by iMod (gen_heap_update m idx _ None with "Hkvs_auth Hkvs_frag") as "[$ $]". *)
+  (* Qed. *)
 
-  Lemma kvs_frag_idx_dupl_false idx k k' w w' :
-    k ⤇(KVS)[ idx ] w -∗ k' ⤇(KVS)[ idx ] w' -∗ False.
-  Proof.
-    iIntros "H1 H2".
-    iDestruct (pointsto_valid_2 with "H1 H2") as %?.
-    destruct H; eapply dfrac_full_exclusive in H; auto.
-  Qed.
+  (* Lemma kvs_frag_idx_dupl_false idx k k' w w' : *)
+  (*   k ⤇(KVS)[ idx ] w -∗ k' ⤇(KVS)[ idx ] w' -∗ False. *)
+  (* Proof. *)
+  (*   iIntros "H1 H2". *)
+  (*   iDestruct (pointsto_valid_2 with "H1 H2") as %?. *)
+  (*   destruct H; eapply dfrac_full_exclusive in H; auto. *)
+  (* Qed. *)
 
-  Lemma kvs_valid_None (m : kvs_map) (idx : nat) :
-    ●(KVS) m -∗
-    idx ⤇(KVS) NONE -∗
-    ⌜ m !! idx = Some None ⌝.
-  Proof.
-    iIntros "Hkvs_auth Hk".
-    by iDestruct (gen_heap_valid with "Hkvs_auth Hk") as "%Hidx'".
-  Qed.
+  (* Lemma kvs_valid_None (m : kvs_physical_map) (idx : nat) : *)
+  (*   ●(KVS) m -∗ *)
+  (*   idx ⤇(KVS) NONE -∗ *)
+  (*   ⌜ m !! idx = Some None ⌝. *)
+  (* Proof. *)
+  (*   iIntros "Hkvs_auth Hk". *)
+  (*   by iDestruct (gen_heap_valid with "Hkvs_auth Hk") as "%Hidx'". *)
+  (* Qed. *)
 
-  Lemma kvs_valid (m : kvs_map) (idx : nat) (k : Z) (w : Word) :
-    ●(KVS) m -∗
-    k ⤇(KVS)[idx] w -∗
-    ⌜ m !! idx = Some (Some (k, w)) ⌝.
-  Proof.
-    iIntros "Hkvs_auth Hk".
-    by iDestruct (gen_heap_valid with "Hkvs_auth Hk") as "%Hidx'".
-  Qed.
+  (* Lemma kvs_valid (m : kvs_physical_map) (idx : nat) (k : Z) (w : Word) : *)
+  (*   ●(KVS) m -∗ *)
+  (*   k ⤇(KVS)[idx] w -∗ *)
+  (*   ⌜ m !! idx = Some (Some (k, w)) ⌝. *)
+  (* Proof. *)
+  (*   iIntros "Hkvs_auth Hk". *)
+  (*   by iDestruct (gen_heap_valid with "Hkvs_auth Hk") as "%Hidx'". *)
+  (* Qed. *)
 
-  Lemma isKVS_valid (m : kvs_map) (lm : kvs_logical_map) (a : Addr) (idx : nat) (k : Z) (w : Word) :
-    isKVS a m lm -∗
-    k ⤇(KVS)[idx] w -∗
-    ⌜ m !! idx = Some (Some (k, w)) ⌝.
-  Proof.
-    iIntros "(%Hwf_kvs & _ & Hkvs_auth & _) Hk".
-    by iDestruct (kvs_valid with "Hkvs_auth Hk") as "%Hidx'".
-  Qed.
+  (* Lemma isKVS_valid (m : kvs_physical_map) (lm : kvs_logical_map) (a : Addr) (idx : nat) (k : Z) (w : Word) : *)
+  (*   isKVS a m lm -∗ *)
+  (*   k ⤇(KVS)[idx] w -∗ *)
+  (*   ⌜ m !! idx = Some (Some (k, w)) ⌝. *)
+  (* Proof. *)
+  (*   iIntros "(%Hwf_kvs & _ & Hkvs_auth & _) Hk". *)
+  (*   by iDestruct (kvs_valid with "Hkvs_auth Hk") as "%Hidx'". *)
+  (* Qed. *)
 
-  Lemma isKVS_valid_None (m : kvs_map) (lm : kvs_logical_map) (a : Addr) (idx : nat) :
-    isKVS a m lm -∗
-    idx ⤇(KVS) NONE -∗
-    ⌜ m !! idx = Some None ⌝.
-  Proof.
-    iIntros "(%Hwf_kvs & _ & Hkvs_auth & _) Hk".
-    by iDestruct (kvs_valid_None with "Hkvs_auth Hk") as "%Hidx'".
-  Qed.
+  (* Lemma isKVS_valid_None (m : kvs_physical_map) (lm : kvs_logical_map) (a : Addr) (idx : nat) : *)
+  (*   isKVS a m lm -∗ *)
+  (*   idx ⤇(KVS) NONE -∗ *)
+  (*   ⌜ m !! idx = Some None ⌝. *)
+  (* Proof. *)
+  (*   iIntros "(%Hwf_kvs & _ & Hkvs_auth & _) Hk". *)
+  (*   by iDestruct (kvs_valid_None with "Hkvs_auth Hk") as "%Hidx'". *)
+  (* Qed. *)
 
-  Lemma isKVS_open_valid (m : kvs_map) (lm : kvs_logical_map) (a : Addr) (idx idx' : nat) (k : Z) (w : Word) :
-    isKVS_open a m lm idx' -∗
-    k ⤇(KVS)[idx] w -∗
-    ⌜ m !! idx = Some (Some (k, w)) ⌝.
-  Proof.
-    iIntros "(%Hwf_kvs & _ & Hkvs_auth & _) Hk".
-    by iDestruct (kvs_valid with "Hkvs_auth Hk") as "%Hidx'".
-  Qed.
+  (* Lemma isKVS_open_valid (m : kvs_physical_map) (lm : kvs_logical_map) (a : Addr) (idx idx' : nat) (k : Z) (w : Word) : *)
+  (*   isKVS_open a m lm idx' -∗ *)
+  (*   k ⤇(KVS)[idx] w -∗ *)
+  (*   ⌜ m !! idx = Some (Some (k, w)) ⌝. *)
+  (* Proof. *)
+  (*   iIntros "(%Hwf_kvs & _ & Hkvs_auth & _) Hk". *)
+  (*   by iDestruct (kvs_valid with "Hkvs_auth Hk") as "%Hidx'". *)
+  (* Qed. *)
 
-  Lemma isKVS_open_valid_None (m : kvs_map) (lm : kvs_logical_map) (a : Addr) (idx idx' : nat) :
-    isKVS_open a m lm idx' -∗
-    idx ⤇(KVS) NONE -∗
-    ⌜ m !! idx = Some None ⌝.
-  Proof.
-    iIntros "(%Hwf_kvs & _ & Hkvs_auth & _) Hk".
-    by iDestruct (kvs_valid_None with "Hkvs_auth Hk") as "%Hidx'".
-  Qed.
+  (* Lemma isKVS_open_valid_None (m : kvs_physical_map) (lm : kvs_logical_map) (a : Addr) (idx idx' : nat) : *)
+  (*   isKVS_open a m lm idx' -∗ *)
+  (*   idx ⤇(KVS) NONE -∗ *)
+  (*   ⌜ m !! idx = Some None ⌝. *)
+  (* Proof. *)
+  (*   iIntros "(%Hwf_kvs & _ & Hkvs_auth & _) Hk". *)
+  (*   by iDestruct (kvs_valid_None with "Hkvs_auth Hk") as "%Hidx'". *)
+  (* Qed. *)
 
-  Lemma open_isKVS_kvs_frag_idx
-    (b : Addr) (m : kvs_map) (lm : kvs_logical_map)
-    (idx : nat) (k : Z) (w : Word) :
-    isKVS b m lm ∗
-    k ⤇(KVS)[idx] w -∗
-    isKVS_open b m lm idx ∗
-    isKVS_entry b idx (Some (k, w)) ∗
-    k ⤇(KVS)[idx] w.
-  Proof.
-    iIntros "( (%Hwf_kvs & %Hwf_alloc & Hkvs_auth & Halloc & HKVS) & Hk)".
-    iDestruct (gen_heap_valid with "Hkvs_auth Hk") as "%Hidx'".
-    rewrite -{2}(insert_id m idx (Some (k,w))); last done.
-    iDestruct (big_sepM_insert_delete with "HKVS") as "[Hkvs_entry HKVS]".
-    iFrame; eauto.
-  Qed.
+  (* Lemma open_isKVS_kvs_frag_idx *)
+  (*   (b : Addr) (m : kvs_physical_map) (lm : kvs_logical_map) *)
+  (*   (idx : nat) (k : Z) (w : Word) : *)
+  (*   isKVS b m lm ∗ *)
+  (*   k ⤇(KVS)[idx] w -∗ *)
+  (*   isKVS_open b m lm idx ∗ *)
+  (*   isKVS_entry b idx (Some (k, w)) ∗ *)
+  (*   k ⤇(KVS)[idx] w. *)
+  (* Proof. *)
+  (*   iIntros "( (%Hwf_kvs & %Hwf_alloc & Hkvs_auth & Halloc & HKVS) & Hk)". *)
+  (*   iDestruct (gen_heap_valid with "Hkvs_auth Hk") as "%Hidx'". *)
+  (*   rewrite -{2}(insert_id m idx (Some (k,w))); last done. *)
+  (*   iDestruct (big_sepM_insert_delete with "HKVS") as "[Hkvs_entry HKVS]". *)
+  (*   iFrame; eauto. *)
+  (* Qed. *)
 
-  Lemma isKVS_indom_idx (m : kvs_map) (lm : kvs_logical_map) (a : Addr) (idx : nat) :
-    idx ∈ dom m ->
-    isKVS a m lm -∗
-    ⌜ 0 <= idx < SIZE_MAP ⌝.
-  Proof.
-    iIntros (Hm_idx) "(%Hwf_kvs & _)"; iPureIntro.
-    by eapply wf_kvs_indom_idx.
-  Qed.
+  (* Lemma isKVS_indom_idx (m : kvs_physical_map) (lm : kvs_logical_map) (a : Addr) (idx : nat) : *)
+  (*   idx ∈ dom m -> *)
+  (*   isKVS a m lm -∗ *)
+  (*   ⌜ 0 <= idx < SIZE_MAP ⌝. *)
+  (* Proof. *)
+  (*   iIntros (Hm_idx) "(%Hwf_kvs & _)"; iPureIntro. *)
+  (*   by eapply wf_kvs_indom_idx. *)
+  (* Qed. *)
 
-  Lemma isKVS_open_indom_idx (m : kvs_map) (lm : kvs_logical_map) (a : Addr) (idx idx' : nat) :
-    idx ∈ dom m ->
-    isKVS_open a m lm idx' -∗
-    ⌜ 0 <= idx < SIZE_MAP ⌝.
-  Proof.
-    iIntros (Hm_idx) "(%Hwf_kvs & _)"; iPureIntro.
-    by eapply wf_kvs_indom_idx.
-  Qed.
+  (* Lemma isKVS_open_indom_idx (m : kvs_physical_map) (lm : kvs_logical_map) (a : Addr) (idx idx' : nat) : *)
+  (*   idx ∈ dom m -> *)
+  (*   isKVS_open a m lm idx' -∗ *)
+  (*   ⌜ 0 <= idx < SIZE_MAP ⌝. *)
+  (* Proof. *)
+  (*   iIntros (Hm_idx) "(%Hwf_kvs & _)"; iPureIntro. *)
+  (*   by eapply wf_kvs_indom_idx. *)
+  (* Qed. *)
 
-  Lemma open_isKVS_kvs_frag_idx_diff
-    (b : Addr) (m : kvs_map) (lm : kvs_logical_map) (idx idx' : nat) (k : Z) (w : Word):
-    0 <= idx' < SIZE_MAP ->
-    idx ≠ idx' ->
-    isKVS b m lm ∗
-    k ⤇(KVS)[ idx ] w -∗
-    ∃ opt_kw',
-      k ⤇(KVS)[ idx ] w ∗
-      isKVS_open b m lm idx' ∗
-      ⌜ m !! idx' = Some opt_kw' ⌝ ∗
-      isKVS_entry b idx' opt_kw' ∗
-      ⌜ match opt_kw' with | Some kw' => k ≠ kw'.1 | None => True end ⌝.
-  Proof.
-    iIntros (Hidx' Hidx_ne) "( (%Hwf_kvs & %Hwf_alloc & Hkvs_auth & Halloc & HKVS) & Hk)".
-    iDestruct (kvs_valid with "Hkvs_auth Hk") as "%Hm_idx".
-    pose proof (wf_kvs_is_Some _ _ Hwf_kvs Hidx') as [ opt_kw' Hm_idx' ].
-    iExists opt_kw'.
-    rewrite -{2}(insert_id m idx' opt_kw'); last done.
-    iDestruct (big_sepM_insert_delete with "HKVS") as "[ Hk' HKVS]".
-    iFrame "∗%".
-    iPureIntro.
-    destruct opt_kw' as [ [k' w'] |]; auto.
-    pose proof (wf_kvs_neq _ _ _ _ _ _ _ Hwf_kvs Hidx_ne Hm_idx Hm_idx') as Hkk'.
-    done.
-  Qed.
+  (* Lemma open_isKVS_kvs_frag_idx_diff *)
+  (*   (b : Addr) (m : kvs_physical_map) (lm : kvs_logical_map) (idx idx' : nat) (k : Z) (w : Word): *)
+  (*   0 <= idx' < SIZE_MAP -> *)
+  (*   idx ≠ idx' -> *)
+  (*   isKVS b m lm ∗ *)
+  (*   k ⤇(KVS)[ idx ] w -∗ *)
+  (*   ∃ opt_kw', *)
+  (*     k ⤇(KVS)[ idx ] w ∗ *)
+  (*     isKVS_open b m lm idx' ∗ *)
+  (*     ⌜ m !! idx' = Some opt_kw' ⌝ ∗ *)
+  (*     isKVS_entry b idx' opt_kw' ∗ *)
+  (*     ⌜ match opt_kw' with | Some kw' => k ≠ kw'.1 | None => True end ⌝. *)
+  (* Proof. *)
+  (*   iIntros (Hidx' Hidx_ne) "( (%Hwf_kvs & %Hwf_alloc & Hkvs_auth & Halloc & HKVS) & Hk)". *)
+  (*   iDestruct (kvs_valid with "Hkvs_auth Hk") as "%Hm_idx". *)
+  (*   pose proof (wf_kvs_is_Some _ _ Hwf_kvs Hidx') as [ opt_kw' Hm_idx' ]. *)
+  (*   iExists opt_kw'. *)
+  (*   rewrite -{2}(insert_id m idx' opt_kw'); last done. *)
+  (*   iDestruct (big_sepM_insert_delete with "HKVS") as "[ Hk' HKVS]". *)
+  (*   iFrame "∗%". *)
+  (*   iPureIntro. *)
+  (*   destruct opt_kw' as [ [k' w'] |]; auto. *)
+  (*   pose proof (wf_kvs_neq _ _ _ _ _ _ _ Hwf_kvs Hidx_ne Hm_idx Hm_idx') as Hkk'. *)
+  (*   done. *)
+  (* Qed. *)
 
-  Lemma open_isKVS_not_alloc
-    (b : Addr) (m : kvs_map) (lm : kvs_logical_map) (umap : kvs_user_map)
-    (idx : nat) (ku kn : Z) :
-    let fkey := kvs_full_key ku kn in
-    is_uint16 kn ->
-    (0 ≤ idx < SIZE_MAP)%Z →
-    kn ∉ dom umap →
-    isKVS b m lm -∗
-    ku ↦(KVS_USER) umap -∗
-    ∃ opt_kwidx,
-      ⌜ m !! idx = Some opt_kwidx ⌝ ∗
-      isKVS_open b m lm idx ∗
-      ku ↦(KVS_USER) umap ∗
-      isKVS_entry b idx opt_kwidx ∗
-      ⌜ match opt_kwidx with | Some kwidx => kwidx.1 ≠ fkey | None => True end ⌝.
-  Proof.
-    intros fkey Hwf_full_key Hidx Hs'.
-    iIntros "(%Hwf_kvs & %Hwf_alloc & Hkvs_auth & Halloc  & HKVS) Hk".
-    iDestruct ( kvs_logical_kvs_valid with "Halloc Hk" ) as "%Hss'".
-    assert (fkey ∉ kvs_keys m) as Hfkey_not_allocated.
-    { apply not_elem_of_dom in Hs'.
-      intro Hcontra.
-      apply elem_of_kvs_keys in Hcontra as (idx'&w&?).
-      ospecialize (Hwf_alloc (ku, kn) w Hwf_full_key).
-      cbn in Hwf_alloc.
-      assert ( kvs_elem_of_kvs m (kvs_full_key ku kn) w ) as Helem.
-      { eexists; eauto. }
-      apply Hwf_alloc in Helem.
-      destruct Helem as (?&?&?); simplify_map_eq.
-    }
-    iFrame.
-    assert ( is_Some (m !! idx) ) as [ opt_kwidx Hm_idx].
-    { apply wf_kvs_is_Some; auto; lia. }
-    rewrite -{1}(insert_id m idx opt_kwidx); last done.
-    iDestruct (big_sepM_insert_delete with "HKVS") as "[Hkvs_entry HKVS]".
-    iFrame "∗%".
-    iPureIntro.
-    destruct opt_kwidx as [ [ kidx widx ]|]; auto.
-    cbn.
-    assert ( kidx ∈ kvs_keys m ) as Hkidx by (apply elem_of_kvs_keys; eauto).
-    set_solver.
-  Qed.
+  (* Lemma open_isKVS_not_alloc *)
+  (*   (b : Addr) (m : kvs_physical_map) (lm : kvs_logical_map) (umap : kvs_user_map) *)
+  (*   (idx : nat) (ku kn : Z) : *)
+  (*   let fkey := kvs_full_key ku kn in *)
+  (*   is_uint16 kn -> *)
+  (*   (0 ≤ idx < SIZE_MAP)%Z → *)
+  (*   kn ∉ dom umap → *)
+  (*   isKVS b m lm -∗ *)
+  (*   ku ↦(KVS_USER) umap -∗ *)
+  (*   ∃ opt_kwidx, *)
+  (*     ⌜ m !! idx = Some opt_kwidx ⌝ ∗ *)
+  (*     isKVS_open b m lm idx ∗ *)
+  (*     ku ↦(KVS_USER) umap ∗ *)
+  (*     isKVS_entry b idx opt_kwidx ∗ *)
+  (*     ⌜ match opt_kwidx with | Some kwidx => kwidx.1 ≠ fkey | None => True end ⌝. *)
+  (* Proof. *)
+  (*   intros fkey Hwf_full_key Hidx Hs'. *)
+  (*   iIntros "(%Hwf_kvs & %Hwf_alloc & Hkvs_auth & Halloc  & HKVS) Hk". *)
+  (*   iDestruct ( kvs_logical_kvs_valid with "Halloc Hk" ) as "%Hss'". *)
+  (*   assert (fkey ∉ kvs_keys m) as Hfkey_not_allocated. *)
+  (*   { apply not_elem_of_dom in Hs'. *)
+  (*     intro Hcontra. *)
+  (*     apply elem_of_kvs_keys in Hcontra as (idx'&w&?). *)
+  (*     ospecialize (Hwf_alloc (ku, kn) w Hwf_full_key). *)
+  (*     cbn in Hwf_alloc. *)
+  (*     assert ( kvs_elem_of_kvs m (kvs_full_key ku kn) w ) as Helem. *)
+  (*     { eexists; eauto. } *)
+  (*     apply Hwf_alloc in Helem. *)
+  (*     destruct Helem as (?&?&?); simplify_map_eq. *)
+  (*   } *)
+  (*   iFrame. *)
+  (*   assert ( is_Some (m !! idx) ) as [ opt_kwidx Hm_idx]. *)
+  (*   { apply wf_kvs_is_Some; auto; lia. } *)
+  (*   rewrite -{1}(insert_id m idx opt_kwidx); last done. *)
+  (*   iDestruct (big_sepM_insert_delete with "HKVS") as "[Hkvs_entry HKVS]". *)
+  (*   iFrame "∗%". *)
+  (*   iPureIntro. *)
+  (*   destruct opt_kwidx as [ [ kidx widx ]|]; auto. *)
+  (*   cbn. *)
+  (*   assert ( kidx ∈ kvs_keys m ) as Hkidx by (apply elem_of_kvs_keys; eauto). *)
+  (*   set_solver. *)
+  (* Qed. *)
 
-  Lemma open_isKVS
-    (b : Addr) (m : kvs_map) (lm : kvs_logical_map)
-    (idx : nat) :
-    (0 ≤ idx < SIZE_MAP)%Z →
-    isKVS b m lm -∗
-    ∃ opt_kwidx,
-      ⌜ m !! idx = Some opt_kwidx ⌝ ∗
-      isKVS_open b m lm idx ∗
-      isKVS_entry b idx opt_kwidx.
-  Proof.
-    intros Hidx.
-    iIntros "(%Hwf_kvs & %Hwf_alloc & Hkvs_auth & Halloc & HKVS)".
-    iFrame.
-    assert ( is_Some (m !! idx) ) as [ opt_kwidx Hm_idx].
-    { apply wf_kvs_is_Some; auto; lia. }
-    rewrite -{1}(insert_id m idx opt_kwidx); last done.
-    iDestruct (big_sepM_insert_delete with "HKVS") as "[Hkvs_entry HKVS]".
-    iFrame "∗%".
-  Qed.
+  (* Lemma open_isKVS *)
+  (*   (b : Addr) (m : kvs_physical_map) (lm : kvs_logical_map) *)
+  (*   (idx : nat) : *)
+  (*   (0 ≤ idx < SIZE_MAP)%Z → *)
+  (*   isKVS b m lm -∗ *)
+  (*   ∃ opt_kwidx, *)
+  (*     ⌜ m !! idx = Some opt_kwidx ⌝ ∗ *)
+  (*     isKVS_open b m lm idx ∗ *)
+  (*     isKVS_entry b idx opt_kwidx. *)
+  (* Proof. *)
+  (*   intros Hidx. *)
+  (*   iIntros "(%Hwf_kvs & %Hwf_alloc & Hkvs_auth & Halloc & HKVS)". *)
+  (*   iFrame. *)
+  (*   assert ( is_Some (m !! idx) ) as [ opt_kwidx Hm_idx]. *)
+  (*   { apply wf_kvs_is_Some; auto; lia. } *)
+  (*   rewrite -{1}(insert_id m idx opt_kwidx); last done. *)
+  (*   iDestruct (big_sepM_insert_delete with "HKVS") as "[Hkvs_entry HKVS]". *)
+  (*   iFrame "∗%". *)
+  (* Qed. *)
 
-  Lemma close_isKVS
-    (b : Addr) (m : kvs_map) (lm : kvs_logical_map) (idx : nat) (opt_kwidx : kvs_entry):
-    m !! idx = Some opt_kwidx ->
-    isKVS_open b m lm idx ∗
-    isKVS_entry b idx opt_kwidx -∗
-    isKVS b m lm.
-  Proof.
-    iIntros (Hidx) "[(%Hwf_kvs & %Hwf_alloc & Hkvs_auth & Halloc & HKVS) Hkvs_entry]"; cbn.
-    iDestruct (big_sepM_delete with "[$HKVS $Hkvs_entry]") as "HKVS"; eauto.
-    iFrame; eauto.
-  Qed.
+  (* Lemma close_isKVS *)
+  (*   (b : Addr) (m : kvs_physical_map) (lm : kvs_logical_map) (idx : nat) (opt_kwidx : kvs_entry): *)
+  (*   m !! idx = Some opt_kwidx -> *)
+  (*   isKVS_open b m lm idx ∗ *)
+  (*   isKVS_entry b idx opt_kwidx -∗ *)
+  (*   isKVS b m lm. *)
+  (* Proof. *)
+  (*   iIntros (Hidx) "[(%Hwf_kvs & %Hwf_alloc & Hkvs_auth & Halloc & HKVS) Hkvs_entry]"; cbn. *)
+  (*   iDestruct (big_sepM_delete with "[$HKVS $Hkvs_entry]") as "HKVS"; eauto. *)
+  (*   iFrame; eauto. *)
+  (* Qed. *)
 
   Lemma NoDup_kvs_keys_elem_of m idx uk mk w idx' uk' mk' w' :
     let f := kvs_full_key uk mk in
@@ -1016,7 +1237,7 @@ Section KVS_preamble.
 
 
   Lemma kvs_synced_logical_kvs_update
-    (m : kvs_map) (lm : kvs_logical_map) (idx : nat) (uk mk : Z) (w : Word) :
+    (m : kvs_physical_map) (lm : kvs_logical_map) (idx : nat) (uk mk : Z) (w : Word) :
     let k := kvs_full_key uk mk in
     NoDup (kvs_keys m) ->
     is_uint16 mk ->
@@ -1036,23 +1257,25 @@ Section KVS_preamble.
         * eexists idx; simplify_map_eq; done.
         * assert ( kvs_elem_of_kvs m (kvs_full_key uk kn) w'' ) as (idx'&?).
           { apply Halloc. eexists;split;eauto.
-            destruct (lm !! uk); eauto.
+            destruct (lm !! uk) eqn:Hlm; cbn;eauto.
             cbn in *;set_solver.
           }
           eexists idx'.
-          destruct (decide (idx = idx')); simplify_eq; cbn in *.
-          ** apply kvs_full_key_inj in H as [? ?]; eauto; simplify_eq.
+          destruct (decide (idx = idx')); simplify_map_eq; cbn in *.
+          ** rewrite Hidx in H; simplify_map_eq.
+             apply kvs_full_key_inj in H as [? ?]; eauto; simplify_eq.
           ** by simplify_map_eq.
       + apply kvs_logical_kvs_insert_lookup_ne in Hlm; simplify_eq; auto.
         assert ( kvs_elem_of_logical_kvs lm ku kn w'') as Hk'.
         { eexists ; split; eauto. }
         eapply Halloc in Hk' as (idx' & Hk).
-        destruct (decide (idx = idx')); simplify_eq; cbn in *.
-        ** apply kvs_full_key_inj in H as [? ?]; eauto; simplify_eq.
+        destruct (decide (idx = idx')); simplify_map_eq; cbn in *.
+        ** rewrite Hidx in Hk; simplify_map_eq.
+           apply kvs_full_key_inj in Hk as [? ?]; eauto; simplify_eq.
         ** by eexists idx'; simplify_map_eq.
     - destruct Hk as (idx' & Hk).
       destruct (decide (idx = idx')); simplify_map_eq; cbn in *.
-      + apply kvs_full_key_inj in H as [? ?]; eauto; simplify_eq.
+      + apply kvs_full_key_inj in Hk as [? ?]; eauto; simplify_eq.
         rewrite /kvs_elem_of_logical_kvs /kvs_logical_kvs_insert.
         destruct (lm !! ku) as [umap|] eqn:Humap ; simplify_map_eq.
         * by eexists; split; eauto; simplify_map_eq.
@@ -1070,77 +1293,77 @@ Section KVS_preamble.
           ** by eexists; split; eauto; simplify_map_eq.
   Qed.
 
-  Lemma isKVS_open_update
-    (a : Addr) (m : kvs_map) (lm : kvs_logical_map) (umap : kvs_user_map)
-    (idx : nat) (uk mk : Z) (w w' : Word) :
-    let k := kvs_full_key uk mk in
-    is_uint16 mk ->
-    isKVS_open a m lm idx -∗
-    k ⤇(KVS)[ idx ] w -∗
-    uk ↦(KVS_USER) umap
-    ==∗
-    isKVS_open a (<[idx:= Some (k, w')]> m) (kvs_logical_kvs_insert lm uk mk w') idx ∗
-    k ⤇(KVS)[ idx ] w' ∗
-    uk ↦(KVS_USER) ( <[mk:=w']> umap )
-  .
-  Proof.
-    intros k Hwf.
-    iIntros "(%Hwf_kvs & %Hwf_alloc & Hkvs_auth & Halloc & HKVS) Hk Humap".
-    iDestruct (kvs_valid with "Hkvs_auth Hk") as "%Hm_idx".
-    iDestruct (kvs_logical_kvs_valid with "Halloc Humap") as "%Hvalid".
-    iMod (kvs_auth_update a m idx _ k _ w' with "Hkvs_auth Hk") as "[$ $]".
-    iMod (kvs_logical_kvs_update uk lm umap (<[mk:=w']> umap) with "Halloc Humap") as "[Halloc_auth Halloc_frag]".
-    eapply (kvs_synced_logical_kvs_update _ _ _ _ _ w') in Hwf_alloc; eauto.
-    2: { by destruct Hwf_kvs. }
-    eapply (wf_kvs_map_update _ _ _ w') in Hwf_kvs; eauto.
-    rewrite delete_insert_eq.
-    iFrame "∗ %".
-    by rewrite /kvs_logical_kvs_insert Hvalid /=.
-  Qed.
+  (* Lemma isKVS_open_update *)
+  (*   (a : Addr) (m : kvs_physical_map) (lm : kvs_logical_map) (umap : kvs_user_map) *)
+  (*   (idx : nat) (uk mk : Z) (w w' : Word) : *)
+  (*   let k := kvs_full_key uk mk in *)
+  (*   is_uint16 mk -> *)
+  (*   isKVS_open a m lm idx -∗ *)
+  (*   k ⤇(KVS)[ idx ] w -∗ *)
+  (*   uk ↦(KVS_USER) umap *)
+  (*   ==∗ *)
+  (*   isKVS_open a (<[idx:= Some (k, w')]> m) (kvs_logical_kvs_insert lm uk mk w') idx ∗ *)
+  (*   k ⤇(KVS)[ idx ] w' ∗ *)
+  (*   uk ↦(KVS_USER) ( <[mk:=w']> umap ) *)
+  (* . *)
+  (* Proof. *)
+  (*   intros k Hwf. *)
+  (*   iIntros "(%Hwf_kvs & %Hwf_alloc & Hkvs_auth & Halloc & HKVS) Hk Humap". *)
+  (*   iDestruct (kvs_valid with "Hkvs_auth Hk") as "%Hm_idx". *)
+  (*   iDestruct (kvs_logical_kvs_valid with "Halloc Humap") as "%Hvalid". *)
+  (*   iMod (kvs_auth_update a m idx _ k _ w' with "Hkvs_auth Hk") as "[$ $]". *)
+  (*   iMod (kvs_logical_kvs_update uk lm umap (<[mk:=w']> umap) with "Halloc Humap") as "[Halloc_auth Halloc_frag]". *)
+  (*   eapply (kvs_synced_logical_kvs_update _ _ _ _ _ w') in Hwf_alloc; eauto. *)
+  (*   2: { by destruct Hwf_kvs. } *)
+  (*   eapply (wf_kvs_physical_map_update _ _ _ w') in Hwf_kvs; eauto. *)
+  (*   rewrite delete_insert_eq. *)
+  (*   iFrame "∗ %". *)
+  (*   by rewrite /kvs_logical_kvs_insert Hvalid /=. *)
+  (* Qed. *)
 
-  Lemma isKVS_open_insert
-    (a : Addr) (m : kvs_map) (lm : kvs_logical_map)
-    (umap : kvs_user_map) (idx : nat) (ku kn : Z) (w : Word) :
-    let k := kvs_full_key ku kn in
-    kn ∉ dom umap →
-    is_uint16 kn ->
-    isKVS_open a m lm idx -∗
-    ku ↦(KVS_USER) umap -∗
-    idx ⤇(KVS) NONE
-    ==∗
-    isKVS_open a (<[idx:= Some (k, w)]> m) (kvs_logical_kvs_insert lm ku kn w) idx ∗
-    ku ↦(KVS_USER) (<[ kn := w ]> umap) ∗
-    k ⤇(KVS)[ idx ] w.
-  Proof.
-    intro k.
-    iIntros (Hs' Hwf_kvs_full_key)
-      "(%Hwf_kvs & %Hwf_alloc & Hkvs_auth & Halloc_auth & HKVS) Halloc_frag Hk".
-    iDestruct (kvs_logical_kvs_valid with "Halloc_auth Halloc_frag") as "%Hvalid".
-    iDestruct (kvs_valid_None with "Hkvs_auth Hk") as "%Hm_idx".
-    iMod (kvs_auth_insert a m idx k w with "Hkvs_auth Hk") as "[$ $]".
-    iMod (kvs_logical_kvs_update ku lm umap (<[kn:=w]> umap) with "Halloc_auth Halloc_frag") as "[Halloc_auth Halloc_frag]".
-    rewrite /kvs_synced_logical_kvs in Hwf_alloc.
-    assert (k ∉ kvs_keys m) as Hk_not_allocated.
-    { apply not_elem_of_dom in Hs'.
-      intro Hcontra.
-      apply elem_of_kvs_keys in Hcontra as (idx'&w'&?).
-      ospecialize (Hwf_alloc (ku, kn) w' Hwf_kvs_full_key).
-      cbn in Hwf_alloc.
-      assert ( kvs_elem_of_kvs m (kvs_full_key ku kn) w' ) as Helem.
-      { eexists; eauto. }
-      apply Hwf_alloc in Helem.
-      destruct Helem as (?&?&?); simplify_map_eq.
-    }
-    eapply (wf_kvs_map_insert _ _ _ w) in Hwf_kvs; eauto.
-    eapply (kvs_synced_logical_kvs_insert _ _ _ _ _ w) in Hwf_alloc; eauto.
-    rewrite delete_insert_eq.
-    subst k.
-    iFrame "∗ %".
-    by rewrite /kvs_logical_kvs_insert Hvalid /=.
-  Qed.
+  (* Lemma isKVS_open_insert *)
+  (*   (a : Addr) (m : kvs_physical_map) (lm : kvs_logical_map) *)
+  (*   (umap : kvs_user_map) (idx : nat) (ku kn : Z) (w : Word) : *)
+  (*   let k := kvs_full_key ku kn in *)
+  (*   kn ∉ dom umap → *)
+  (*   is_uint16 kn -> *)
+  (*   isKVS_open a m lm idx -∗ *)
+  (*   ku ↦(KVS_USER) umap -∗ *)
+  (*   idx ⤇(KVS) NONE *)
+  (*   ==∗ *)
+  (*   isKVS_open a (<[idx:= Some (k, w)]> m) (kvs_logical_kvs_insert lm ku kn w) idx ∗ *)
+  (*   ku ↦(KVS_USER) (<[ kn := w ]> umap) ∗ *)
+  (*   k ⤇(KVS)[ idx ] w. *)
+  (* Proof. *)
+  (*   intro k. *)
+  (*   iIntros (Hs' Hwf_kvs_full_key) *)
+  (*     "(%Hwf_kvs & %Hwf_alloc & Hkvs_auth & Halloc_auth & HKVS) Halloc_frag Hk". *)
+  (*   iDestruct (kvs_logical_kvs_valid with "Halloc_auth Halloc_frag") as "%Hvalid". *)
+  (*   iDestruct (kvs_valid_None with "Hkvs_auth Hk") as "%Hm_idx". *)
+  (*   iMod (kvs_auth_insert a m idx k w with "Hkvs_auth Hk") as "[$ $]". *)
+  (*   iMod (kvs_logical_kvs_update ku lm umap (<[kn:=w]> umap) with "Halloc_auth Halloc_frag") as "[Halloc_auth Halloc_frag]". *)
+  (*   rewrite /kvs_synced_logical_kvs in Hwf_alloc. *)
+  (*   assert (k ∉ kvs_keys m) as Hk_not_allocated. *)
+  (*   { apply not_elem_of_dom in Hs'. *)
+  (*     intro Hcontra. *)
+  (*     apply elem_of_kvs_keys in Hcontra as (idx'&w'&?). *)
+  (*     ospecialize (Hwf_alloc (ku, kn) w' Hwf_kvs_full_key). *)
+  (*     cbn in Hwf_alloc. *)
+  (*     assert ( kvs_elem_of_kvs m (kvs_full_key ku kn) w' ) as Helem. *)
+  (*     { eexists; eauto. } *)
+  (*     apply Hwf_alloc in Helem. *)
+  (*     destruct Helem as (?&?&?); simplify_map_eq. *)
+  (*   } *)
+  (*   eapply (wf_kvs_physical_map_insert _ _ _ w) in Hwf_kvs; eauto. *)
+  (*   eapply (kvs_synced_logical_kvs_insert _ _ _ _ _ w) in Hwf_alloc; eauto. *)
+  (*   rewrite delete_insert_eq. *)
+  (*   subst k. *)
+  (*   iFrame "∗ %". *)
+  (*   by rewrite /kvs_logical_kvs_insert Hvalid /=. *)
+  (* Qed. *)
 
   Local Lemma kvs_synced_logical_kvs_delete_1
-    (m : kvs_map) (lm : kvs_logical_map) (idx : nat) (uk mk uk' mk' : Z) (w w' : Word) :
+    (m : kvs_physical_map) (lm : kvs_logical_map) (idx : nat) (uk mk uk' mk' : Z) (w w' : Word) :
     let fkey := kvs_full_key uk mk in
     is_uint16 mk ->
     m !! idx = Some (Some (fkey, w)) ->
@@ -1163,18 +1386,20 @@ Section KVS_preamble.
       apply Halloc in Helem as (idx'&Hidx').
       eexists idx'.
       destruct (decide (idx = idx')); simplify_map_eq; cbn in *; auto.
-      apply kvs_full_key_inj in H as [_ ->]; eauto; done.
+      rewrite Hidx in Hidx'; simplify_map_eq.
+      apply kvs_full_key_inj in Hidx' as [_ ->]; eauto; done.
     - apply kvs_logical_kvs_delete_lookup_ne in Huk'; auto; simplify_map_eq.
       assert (∃ umap : kvs_user_map, lm !! uk' = Some umap ∧ umap !! mk' = Some w') as IH.
       { exists umap; split; auto. }
       apply (Halloc (uk', mk') w' Hwf_full_key') in IH as (idx'&Hidx').
       destruct (decide (idx = idx')); simplify_map_eq; cbn in *; auto.
-      * apply kvs_full_key_inj in H as [-> ->] ;eauto; done.
+      * rewrite Hidx in Hidx'; simplify_map_eq.
+        apply kvs_full_key_inj in Hidx' as [-> ->] ;eauto; done.
       * by exists idx'; simplify_map_eq.
   Qed.
 
   Local Lemma kvs_synced_logical_kvs_delete_2
-    (m : kvs_map) (lm : kvs_logical_map) (idx : nat) (uk mk uk' mk' : Z) (w w' : Word) :
+    (m : kvs_physical_map) (lm : kvs_logical_map) (idx : nat) (uk mk uk' mk' : Z) (w w' : Word) :
     let fkey := kvs_full_key uk mk in
     is_uint16 mk ->
     m !! idx = Some (Some (fkey, w)) ->
@@ -1195,7 +1420,7 @@ Section KVS_preamble.
 
     apply IH' in IHm' as (umap' & Humap' & Hmk'_in_umap').
     assert (kvs_full_key uk mk ∈ kvs_keys m) as IHm.
-    { apply elem_of_kvs_keys; eauto. }
+    { apply elem_of_kvs_keys; eexists _,_; eauto. }
     rewrite /kvs_logical_kvs_delete.
     destruct (decide (uk = uk')); simplify_map_eq; cycle 1.
     { exists umap'; split; simplify_map_eq;eauto. }
@@ -1206,7 +1431,7 @@ Section KVS_preamble.
     destruct Hnodup as [ | ]; done.
   Qed.
 
-  Lemma kvs_synced_logical_kvs_delete (m : kvs_map) (lm : kvs_logical_map) (idx : nat) (uk mk : Z) (w : Word) :
+  Lemma kvs_synced_logical_kvs_delete (m : kvs_physical_map) (lm : kvs_logical_map) (idx : nat) (uk mk : Z) (w : Word) :
     let fkey := kvs_full_key uk mk in
     NoDup (kvs_keys m) ->
     is_uint16 mk ->
@@ -1223,7 +1448,7 @@ Section KVS_preamble.
   Qed.
 
   Lemma NoDup_kvs_keys_delete
-    (m : kvs_map) (idx : nat)  :
+    (m : kvs_physical_map) (idx : nat)  :
     NoDup (kvs_keys m) ->
     NoDup (kvs_keys (<[idx:=None]> m)).
   Proof.
@@ -1243,7 +1468,7 @@ Section KVS_preamble.
         apply NoDup_cons in Hnodup as [ Hk' Hnodup ]; auto.
         rewrite kvs_keys_insert_Some; simplify_map_eq; auto.
         apply NoDup_cons; split ; auto.
-        intro Hk. apply elem_of_kvs_keys in Hk as (idx_k&?&?); simplify_eq.
+        intro Hk. apply elem_of_kvs_keys in Hk as (?&idx_k&?); simplify_eq.
         destruct (decide (idx_k = idx)); simplify_map_eq.
         apply Hk'.
         apply elem_of_kvs_keys; eexists _,_ ; eauto.
@@ -1251,10 +1476,10 @@ Section KVS_preamble.
         rewrite kvs_keys_insert_None; simplify_map_eq; auto.
   Qed.
 
-  Lemma wf_kvs_map_delete (m : kvs_map) (idx : nat) (k : Z) :
+  Lemma wf_kvs_physical_map_delete (m : kvs_physical_map) (idx : nat) (k : Z) :
     (is_Some (m !! idx)) ->
-    wf_kvs_map m ->
-    wf_kvs_map (<[idx:=None]> m).
+    wf_kvs_physical_map m ->
+    wf_kvs_physical_map (<[idx:=None]> m).
   Proof.
     intros [w' Hidx] (Hkvs_dom & Hkvs_unique).
     split.
@@ -1265,53 +1490,44 @@ Section KVS_preamble.
     - eapply NoDup_kvs_keys_delete; eauto.
   Qed.
 
-  Lemma isKVS_open_delete (a : Addr) (m : kvs_map) (lm : kvs_logical_map) (umap : kvs_user_map)
-    (idx : nat) (uk mk : Z) (w : Word) :
-    let k := kvs_full_key uk mk in
-    is_uint16 mk ->
-    isKVS_open a m lm idx -∗
-    uk ↦(KVS_USER) umap -∗
-    k ⤇(KVS)[ idx ] w
-    ==∗
-    isKVS_open a (<[idx:=None]> m) (kvs_logical_kvs_delete lm uk mk) idx ∗
-    uk ↦(KVS_USER) (delete mk umap) ∗
-    idx ⤇(KVS) NONE.
-  Proof.
-    intro k.
-    iIntros (Hwf_kvs_full_key)
-      "(%Hwf_kvs & %Hwf_alloc & Hkvs_auth & Halloc_auth & HKVS) Halloc_frag Hk".
-    iDestruct (kvs_logical_kvs_valid with "Halloc_auth Halloc_frag") as "%Hvalid".
-    iDestruct (kvs_valid with "Hkvs_auth Hk") as "%Hm_idx".
-    iMod (kvs_auth_delete a m idx _ _ with "Hkvs_auth Hk") as "[$ $]".
+  (* Lemma isKVS_open_delete (a : Addr) (m : kvs_physical_map) (lm : kvs_logical_map) (umap : kvs_user_map) *)
+  (*   (idx : nat) (uk mk : Z) (w : Word) : *)
+  (*   let k := kvs_full_key uk mk in *)
+  (*   is_uint16 mk -> *)
+  (*   isKVS_open a m lm idx -∗ *)
+  (*   uk ↦(KVS_USER) umap -∗ *)
+  (*   k ⤇(KVS)[ idx ] w *)
+  (*   ==∗ *)
+  (*   isKVS_open a (<[idx:=None]> m) (kvs_logical_kvs_delete lm uk mk) idx ∗ *)
+  (*   uk ↦(KVS_USER) (delete mk umap) ∗ *)
+  (*   idx ⤇(KVS) NONE. *)
+  (* Proof. *)
+  (*   intro k. *)
+  (*   iIntros (Hwf_kvs_full_key) *)
+  (*     "(%Hwf_kvs & %Hwf_alloc & Hkvs_auth & Halloc_auth & HKVS) Halloc_frag Hk". *)
+  (*   iDestruct (kvs_logical_kvs_valid with "Halloc_auth Halloc_frag") as "%Hvalid". *)
+  (*   iDestruct (kvs_valid with "Hkvs_auth Hk") as "%Hm_idx". *)
+  (*   iMod (kvs_auth_delete a m idx _ _ with "Hkvs_auth Hk") as "[$ $]". *)
 
-    iMod ( kvs_logical_kvs_update uk lm umap (delete mk umap) with "Halloc_auth Halloc_frag") as "[Halloc_auth Halloc_frag]".
-    assert (NoDup (kvs_keys m)) as Hnodup by ( by destruct Hwf_kvs ).
-    rewrite /kvs_synced_logical_kvs in Hwf_alloc.
-    eapply (wf_kvs_map_delete _ _) in Hwf_kvs; eauto.
-    eapply (kvs_synced_logical_kvs_delete _ _ _ _ _ w) in Hwf_alloc; eauto.
-    rewrite delete_insert_eq.
-    subst k.
-    iFrame "∗ %".
-    by rewrite /kvs_logical_kvs_delete Hvalid /=.
-  Qed.
+  (*   iMod ( kvs_logical_kvs_update uk lm umap (delete mk umap) with "Halloc_auth Halloc_frag") as "[Halloc_auth Halloc_frag]". *)
+  (*   assert (NoDup (kvs_keys m)) as Hnodup by ( by destruct Hwf_kvs ). *)
+  (*   rewrite /kvs_synced_logical_kvs in Hwf_alloc. *)
+  (*   eapply (wf_kvs_physical_map_delete _ _) in Hwf_kvs; eauto. *)
+  (*   eapply (kvs_synced_logical_kvs_delete _ _ _ _ _ w) in Hwf_alloc; eauto. *)
+  (*   rewrite delete_insert_eq. *)
+  (*   subst k. *)
+  (*   iFrame "∗ %". *)
+  (*   by rewrite /kvs_logical_kvs_delete Hvalid /=. *)
+  (* Qed. *)
 
 End KVS_preamble.
 
-Definition kvs_user_map_auth `{kvsG} (uk : Z) (m : kvs_user_map) : iProp Σ := uk ↦(KVS_USER) m.
-Definition kvs_user_map_frag `{kvsG} (uk mk : Z) ( w : Word ) : iProp Σ := kvs_full_key uk mk ⤇(KVS) w.
+(* Definition kvs_user_map_auth `{kvsG} (uk : Z) (m : kvs_user_map) : iProp Σ := uk ↦(KVS_USER) m. *)
+(* Definition kvs_user_map_frag `{kvsG} (uk mk : Z) ( w : Word ) : iProp Σ := kvs_full_key uk mk ⤇(KVS) w. *)
 
-Notation "'◯↪KVS[' uk ']' m" := (kvs_user_map_auth uk m)%I (at level 20) : bi_scope.
-Notation "mk '↦(KVS)[' uk ']' w" := (kvs_user_map_frag uk mk w)%I (at level 20) : bi_scope.
-Notation "mk '↦(KVS)[' uk ']' -" := (∃ w, mk ↦(KVS)[ uk ] w)%I (at level 20) : bi_scope.
-
-Class kvs_namespaces :=
-  {
-    Nkvs : namespace;
-    Nkvs_otype : namespace;
-    Nkvs_exp_tbl : namespace;
-    Nkvs_namespaces_disjoint :
-    Nkvs ## Nkvs_otype ∧ Nkvs ## Nkvs_exp_tbl ∧ Nkvs_otype ## Nkvs_exp_tbl
-  }.
+(* Notation "'◯↪KVS[' uk ']' m" := (kvs_user_map_auth uk m)%I (at level 20) : bi_scope. *)
+(* Notation "mk '↦(KVS)[' uk ']' w" := (kvs_user_map_frag uk mk w)%I (at level 20) : bi_scope. *)
+(* Notation "mk '↦(KVS)[' uk ']' -" := (∃ w, mk ↦(KVS)[ uk ] w)%I (at level 20) : bi_scope. *)
 
 
 Section KVS_preamble_public.
@@ -1338,9 +1554,8 @@ Section KVS_preamble_public.
       (* Payload contains the user key *)
       a ↦ₐ WInt uk ∗
       (* KVS resources *)
-      ◯↪KVS[ uk ] m ∗
-      ([∗ map] mk↦w ∈ m, mk ↦(KVS)[uk] w ∗
-                         (∀ W' , ⌜ related_sts_priv_world W W' ⌝ -∗ interp W' C w )
+      uk ↦(LKVS) m ∗
+      ([∗ map] mk↦w ∈ m, (∀ W' , ⌜ related_sts_priv_world W W' ⌝ -∗ interp W' C w )
       ).
 
   Program Definition kvs_otype_prop
@@ -1366,7 +1581,7 @@ Section KVS_preamble_public.
     iDestruct "Hot_kvs" as "(%ku & %a & %s & % & % & ? & ? & Hs)".
     iExists ku, a, s; iFrame "∗%".
     iApply (big_sepM_impl with "Hs").
-    iModIntro; iIntros (???) "($ & H)".
+    iModIntro; iIntros (???) "H".
     iIntros (W'' Hrelated_W'_W'').
     iApply "H".
     iPureIntro.
@@ -1377,35 +1592,34 @@ Section KVS_preamble_public.
     let imports :=
       kvs_imports b_switcher e_switcher a_switcher_call ot_switcher
     in
-    ∃ (m : kvs_map) (s : kvs_logical_map),
       [[ KVS_pcc_b , KVS_pcc_b' ]] ↦ₐ [[ imports ]] ∗
       codefrag KVS_pcc_b' kvs_service_instrs ∗
-      isKVS KVS_cgp_b m s ∗
+      logical_kvs_inv KVS_cgp_b ∗
       seal_pred KVS_OTYPE kvs_otype_propC.
 
-  Lemma kvs_pointsto_valid
-    (a : Addr) (mkvs : kvs_map) (lm : kvs_logical_map)
-    (m : kvs_user_map) (uk mk : Z) (w : Word) :
-      is_uint16 mk ->
-      isKVS a mkvs lm -∗
-      ◯↪KVS[ uk ] m -∗
-      mk ↦(KVS)[uk] w
-      -∗
-      ⌜ m !! mk = Some w ⌝.
-  Proof.
-    iIntros (Hwf_key) "(%Hwk_kvs & %Hsynced & Hkvs & Hlkvs & _) Hm Hmk".
-    rewrite /kvs_user_map_auth /kvs_user_map_frag.
-    iDestruct ( kvs_logical_kvs_valid with "Hlkvs Hm") as "%Huk".
-    iDestruct "Hmk" as "[%idx Hmk]".
-    iDestruct (kvs_valid with "Hkvs Hmk" ) as "%Hidx".
-    specialize (Hsynced (uk,mk) w Hwf_key); cbn in *.
-    assert ( kvs_elem_of_kvs mkvs (kvs_full_key uk mk) w ) as H by (eexists;eauto).
-    apply Hsynced in H as (?&?&?); simplify_eq.
-    done.
-  Qed.
+  (* Lemma kvs_pointsto_valid *)
+  (*   (a : Addr) (mkvs : kvs_physical_map) (lm : kvs_logical_map) *)
+  (*   (m : kvs_user_map) (uk mk : Z) (w : Word) : *)
+  (*     is_uint16 mk -> *)
+  (*     isKVS a mkvs lm -∗ *)
+  (*     ◯↪KVS[ uk ] m -∗ *)
+  (*     mk ↦(KVS)[uk] w *)
+  (*     -∗ *)
+  (*     ⌜ m !! mk = Some w ⌝. *)
+  (* Proof. *)
+  (*   iIntros (Hwf_key) "(%Hwk_kvs & %Hsynced & Hkvs & Hlkvs & _) Hm Hmk". *)
+  (*   rewrite /kvs_user_map_auth /kvs_user_map_frag. *)
+  (*   iDestruct ( kvs_logical_kvs_valid with "Hlkvs Hm") as "%Huk". *)
+  (*   iDestruct "Hmk" as "[%idx Hmk]". *)
+  (*   iDestruct (kvs_valid with "Hkvs Hmk" ) as "%Hidx". *)
+  (*   specialize (Hsynced (uk,mk) w Hwf_key); cbn in *. *)
+  (*   assert ( kvs_elem_of_kvs mkvs (kvs_full_key uk mk) w ) as H by (eexists;eauto). *)
+  (*   apply Hsynced in H as (?&?&?); simplify_eq. *)
+  (*   done. *)
+  (* Qed. *)
 
 End KVS_preamble_public.
 
-Global Opaque kvs_map_init.
-Global Opaque kvs_user_map_auth.
-Global Opaque kvs_user_map_frag.
+Global Opaque kvs_physical_map_init.
+(* Global Opaque kvs_user_map_auth. *)
+(* Global Opaque kvs_user_map_frag. *)
